remove trait/class from validation proof

cedar-dafny/validation/thm/model.dfy
@@ -22,6 +22,7 @@ include "base.dfy"
 module validation.thm.model {
   import opened def
   import opened def.core
+  import opened def.engine
   import opened types
   import opened subtyping
   import opened base
@@ -38,7 +39,7 @@ module validation.thm.model {
     exists i :: 0 <= i < |es| && es[i].0 == k
   }
 
-  ghost function {:opaque true} LastOfKey<K,V>(k: K, es: seq<(K,V)>): (res: V)
+  opaque ghost function LastOfKey<K,V>(k: K, es: seq<(K,V)>): (res: V)
     requires KeyExists(k,es)
     ensures exists i :: 0 <= i < |es| && es[i].0 == k && es[i].1 == res && (forall j :: i < j < |es| ==> es[j].0 != k)
   {
@@ -64,1222 +65,1008 @@ module validation.thm.model {
     ensures Evaluator(r,s).interpretSet(es).Err? ==> exists i :: 0 <= i < |es| && Evaluator(r,s).interpret(es[i]).Err? && Evaluator(r,s).interpret(es[i]).error == Evaluator(r,s).interpretSet(es).error && (forall j :: 0 <= j < i ==> Evaluator(r,s).interpret(es[j]).Ok?);
   {}
 
-  // An implementation of the SemanticModel trait is a model of Cedar.
-  // It consists of two main predicates: InstanceOfType and IsSafe, as well as
-  // compatability lemmata about the predicates.
-  //
-  // IsSafe(r, s, e, t) says that when evaluated with Request `q` and EntityStore `s`,
-  // evaluating Expr `e` will result in a Value of type `t`.
-  //
-  // The compatability lemmata are obtained by taking the Cedar typing rules, and
-  // replacing the typing relation with the expression safety relation.
-  // For example, in Cedar, when e: Bool and e': False, then e && e': False.
-  // This is mirrored by the required lemma `AndRShortSafe`, shown below.
-  //
-  //  lemma AndRShortSafe(r: Request, s: EntityStore, e: Expr, e': Expr)
-  //    requires IsSafe(r,s,e,Type.Bool(AnyBool))
-  //    requires IsSafe(r,s,e',Type.Bool(False))
-  //    ensures IsSafe(r,s,And(e,e'),Type.Bool(False))
-  //
-  // Every Cedar typing rule has a related compatability lemma. The upshot of this
-  // is that we can prove, by induction on the typing relation e: t, that
-  // model.IsSafe(_,_,e,t), for any model: SemanticModel.
+  // ----- Semantic model of Cedar ----- //
 
-  // The SemanticModel construction can also be thought of as a way of axiomatizing
+  // The semantic model construction can be thought of as a way of axiomatizing
   // the behavior of the evaluator that's necessary to prove soundness. When we
   // prove soundness, hiding these properties behind the axiomatic interface
   // of a trait improves the performance of the Dafny verifier significantly.
-  trait SemanticModel {
-    ghost predicate IsSafe(r: Request, s: EntityStore, e: Expr, t: Type)
 
-    // stronger version of `IsSafe` that disallows errors
-    ghost predicate IsSafeStrong(r: Request, s: EntityStore, e: Expr, t: Type)
-
-    // useful shorthands
-    ghost predicate IsTrue (r: Request, s: EntityStore, e: Expr) {
-      IsSafe(r,s,e,Type.Bool(True))
-    }
-    ghost predicate IsFalse (r: Request, s: EntityStore, e: Expr) {
-      IsSafe(r,s,e,Type.Bool(False))
-    }
-    ghost predicate GetAttrSafe (r: Request, s: EntityStore, e: Expr, k: Attr) {
-      IsTrue(r,s,HasAttr(e,k))
-    }
-    ghost predicate IsTrueStrong (r: Request, s: EntityStore, e: Expr) {
-      IsSafeStrong(r,s,e,Type.Bool(True))
-    }
-    ghost predicate IsFalseStrong (r: Request, s: EntityStore, e: Expr) {
-      IsSafeStrong(r,s,e,Type.Bool(False))
-    }
-
-    lemma IsTrueStrongImpliesIsTrue(r: Request, s: EntityStore, e: Expr)
-      requires IsTrueStrong(r,s,e)
-      ensures IsTrue(r,s,e)
-
-    lemma IsTrueImpliesIsTrueStrong(r: Request, s: EntityStore, e: Expr, t: Type)
-      requires IsSafeStrong(r,s,e,t)
-      requires IsTrue(r,s,e)
-      ensures IsTrueStrong(r,s,e)
-
-    lemma NotTrueImpliesFalse(r: Request, s: EntityStore, e: Expr, bt: BoolType)
-      requires IsSafe(r,s,e,Type.Bool(bt))
-      requires !IsTrue(r,s,e)
-      ensures IsFalse(r,s,e)
-
-    lemma FalseImpliesNotTrueStrong(r: Request, s: EntityStore, e: Expr)
-      requires IsFalse(r,s,e)
-      ensures !IsTrueStrong(r,s,e)
-
-    ghost predicate SemanticSubty(t1: Type, t2: Type) {
-      forall v :: InstanceOfType(v,t1) ==> InstanceOfType(v,t2)
-    }
-
-    ghost predicate SemanticUB(t1: Type, t2: Type, ub: Type) {
-      SemanticSubty(t1,ub) && SemanticSubty(t2,ub)
-    }
-
-    lemma SubtyCompat(t1: Type, t2: Type)
-      requires subty(t1,t2)
-      ensures SemanticSubty(t1,t2)
-
-    lemma SemSubtyTransportVal(t: Type, t': Type, v: Value)
-      requires SemanticSubty(t,t')
-      requires InstanceOfType(v,t)
-      ensures InstanceOfType(v,t')
-    {}
-
-    lemma SemSubtyTransport(r: Request, s: EntityStore, e: Expr, t: Type, t': Type)
-      requires SemanticSubty(t,t')
-      requires IsSafe(r,s,e,t)
-      ensures IsSafe(r,s,e,t')
-
-    lemma PrincipalIsSafe(r: Request, s: EntityStore, t: Type)
-      requires InstanceOfType(Value.EntityUID(r.principal),t)
-      ensures IsSafe(r,s,Var(Principal),t)
-
-    lemma ActionIsSafe(r: Request, s: EntityStore, t: Type)
-      requires InstanceOfType(Value.EntityUID(r.action),t)
-      ensures IsSafe(r,s,Var(Action),t)
-
-    lemma ResourceIsSafe(r: Request, s: EntityStore, t: Type)
-      requires InstanceOfType(Value.EntityUID(r.resource),t)
-      ensures IsSafe(r,s,Var(Resource),t)
-
-    lemma ContextIsSafe(r: Request, s: EntityStore, t: Type)
-      requires InstanceOfType(Value.Record(r.context),t)
-      ensures IsSafe(r,s,Var(Context),t)
-
-    lemma PrimSafeLift(r: Request, s: EntityStore, p: Primitive, t: Type)
-      requires InstanceOfType(Value.Primitive(p),t)
-      ensures IsSafe(r,s,Expr.PrimitiveLit(p),t)
-
-    lemma PrimSafeAtInferredType(p: Primitive)
-      ensures InstanceOfType(Value.Primitive(p),typeOfPrim(p))
-
-    lemma EqIsSafe(r: Request, s: EntityStore, e: Expr, e': Expr, t: Type, t': Type)
-      requires IsSafe(r,s,e,t)
-      requires IsSafe(r,s,e',t')
-      ensures IsSafe(r,s,BinaryApp(BinaryOp.Eq,e,e'),Type.Bool(AnyBool))
-
-    lemma EqFalseIsSafe(r: Request, s: EntityStore, e: Expr, e': Expr, lub: EntityLUB, lub': EntityLUB)
-      requires IsSafe(r,s,e,Type.Entity(lub))
-      requires IsSafe(r,s,e',Type.Entity(lub'))
-      requires lub.disjoint(lub')
-      ensures IsFalse(r,s,BinaryApp(BinaryOp.Eq,e,e'))
-
-    lemma EqEntitySameSafe(r: Request, s: EntityStore, E: EntityUID)
-      ensures IsTrue(r,s,Expr.BinaryApp(BinaryOp.Eq,PrimitiveLit(Primitive.EntityUID(E)),PrimitiveLit(Primitive.EntityUID(E))))
-
-    lemma EqEntityDiffSafe(r: Request, s: EntityStore, E: EntityUID, E': EntityUID)
-      requires E != E'
-      ensures IsFalse(r,s,Expr.BinaryApp(BinaryOp.Eq,PrimitiveLit(Primitive.EntityUID(E)),PrimitiveLit(Primitive.EntityUID(E'))))
-
-    lemma AndLShortSafe(r: Request, s: EntityStore, e: Expr, e': Expr)
-      requires IsFalse(r,s,e)
-      ensures IsFalse(r,s,And(e,e'))
-
-    lemma AndRShortSafe(r: Request, s: EntityStore, e: Expr, e': Expr)
-      requires IsSafe(r,s,e,Type.Bool(AnyBool))
-      requires IsFalse(r,s,e')
-      ensures IsFalse(r,s,And(e,e'))
-
-    lemma AndLRetSafe(r: Request, s: EntityStore, e: Expr, e': Expr, t: Type)
-      requires IsSafe(r,s,e,t)
-      requires IsTrue(r,s,e')
-      requires SemanticSubty(t,Type.Bool(AnyBool))
-      ensures IsSafe(r,s,And(e,e'),t)
-
-    lemma AndSafe(r: Request, s: EntityStore, e: Expr, e': Expr)
-      requires IsSafe(r,s,e,Type.Bool(AnyBool))
-      requires IsSafe(r,s,e',Type.Bool(AnyBool))
-      ensures IsSafe(r,s,And(e,e'),Type.Bool(AnyBool))
-
-    lemma AndTrueStrong(r: Request, s: EntityStore, e1: Expr, e2: Expr)
-      requires IsTrue(r,s,e1)
-      requires IsTrueStrong(r,s,And(e1,e2))
-      ensures IsTrueStrong(r,s,e2)
-
-    lemma AndError(r: Request, s: EntityStore, e1: Expr, e2: Expr, t: Type, tnew: Type)
-      requires IsSafe(r,s,e1,t)
-      requires !IsSafeStrong(r,s,e1,t)
-      ensures IsSafe(r,s,And(e1,e2),tnew)
-      ensures !IsSafeStrong(r,s,And(e1,e2),tnew)
-
-    lemma OrLShortSafe(r: Request, s: EntityStore, e: Expr, e': Expr)
-      requires IsTrue(r,s,e)
-      ensures IsTrue(r,s,Or(e,e'))
-
-    lemma OrRShortSafe(r: Request, s: EntityStore, e: Expr, e': Expr)
-      requires IsSafe(r,s,e,Type.Bool(AnyBool))
-      requires IsTrue(r,s,e')
-      ensures IsTrue(r,s,Or(e,e'))
-
-    lemma OrLRetSafe(r: Request, s: EntityStore, e: Expr, e': Expr, t: Type)
-      requires IsSafe(r,s,e,t)
-      requires IsFalse(r,s,e')
-      requires SemanticSubty(t,Type.Bool(AnyBool))
-      ensures IsSafe(r,s,Or(e,e'),t)
-
-    lemma OrRRetSafe(r: Request, s: EntityStore, e: Expr, e': Expr, t: Type)
-      requires IsFalse(r,s,e)
-      requires IsSafe(r,s,e',t)
-      requires SemanticSubty(t,Type.Bool(AnyBool))
-      ensures IsSafe(r,s,Or(e,e'),t)
-
-    lemma OrSafe(r: Request, s: EntityStore, e: Expr, e': Expr)
-      requires IsSafe(r,s,e,Type.Bool(AnyBool))
-      requires IsSafe(r,s,e',Type.Bool(AnyBool))
-      ensures IsSafe(r,s,Or(e,e'),Type.Bool(AnyBool))
-
-    lemma OrTrueStrong(r: Request, s: EntityStore, e1: Expr, e2: Expr)
-      requires IsTrueStrong(r,s,Or(e1,e2))
-      ensures IsTrueStrong(r,s,e1) || IsTrueStrong(r,s,e2)
-
-    lemma NotTrueSafe(r: Request, s: EntityStore, e: Expr)
-      requires IsTrue(r,s,e)
-      ensures IsFalse(r,s,UnaryApp(Not,e))
-
-    lemma NotFalseSafe(r: Request, s: EntityStore, e: Expr)
-      requires IsFalse(r,s,e)
-      ensures IsTrue(r,s,UnaryApp(Not,e))
-
-    lemma NotSafe(r: Request, s: EntityStore, e: Expr)
-      requires IsSafe(r,s,e,Type.Bool(AnyBool))
-      ensures IsSafe(r,s,UnaryApp(Not,e),Type.Bool(AnyBool))
-
-    lemma NegSafe(r: Request, s: EntityStore, e: Expr)
-      requires IsSafe(r,s,e,Type.Int)
-      ensures IsSafe(r,s,UnaryApp(Neg,e),Type.Int)
-
-    lemma MulBySafe(r: Request, s: EntityStore, e: Expr, i: int)
-      requires IsSafe(r,s,e,Type.Int)
-      ensures IsSafe(r,s,UnaryApp(MulBy(i),e),Type.Int)
-
-    lemma IteTrueSafe(r: Request, s: EntityStore, e: Expr, e1: Expr, e2: Expr, t: Type)
-      requires IsTrue(r,s,e)
-      requires IsSafe(r,s,e1,t)
-      ensures IsSafe(r,s,If(e,e1,e2),t)
-
-    lemma IteFalseSafe(r: Request, s: EntityStore, e: Expr, e1: Expr, e2: Expr, t: Type)
-      requires IsFalse(r,s,e)
-      requires IsSafe(r,s,e2,t)
-      ensures IsSafe(r,s,If(e,e1,e2),t)
-
-    lemma IteTrueStrongTrue(r: Request, s: EntityStore, e1: Expr, e2: Expr, e3: Expr)
-      requires IsTrue(r,s,e1)
-      requires IsTrueStrong(r,s,If(e1,e2,e3))
-      ensures IsTrueStrong(r,s,e2)
-
-    lemma IteTrueStrongFalse(r: Request, s: EntityStore, e1: Expr, e2: Expr, e3: Expr)
-      requires IsFalse(r,s,e1)
-      requires IsTrueStrong(r,s,If(e1,e2,e3))
-      ensures IsTrueStrong(r,s,e3)
-
-    lemma IteError(r: Request, s: EntityStore, e1: Expr, e2: Expr, e3: Expr, t: Type, tnew: Type)
-      requires IsSafe(r,s,e1,t)
-      requires !IsSafeStrong(r,s,e1,t)
-      ensures IsSafe(r,s,If(e1,e2,e3),tnew)
-      ensures !IsSafeStrong(r,s,If(e1,e2,e3),tnew)
-
-    lemma ContainsSetSafe(r: Request, s: EntityStore, e: Expr, e': Expr, t1: Type, t2: Type)
-      requires IsSafe(r,s,e,Type.Set(t1))
-      requires IsSafe(r,s,e',t2)
-      ensures IsSafe(r,s,BinaryApp(Contains,e,e'),Type.Bool(AnyBool))
-
-    lemma LikeSafe(r: Request, s: EntityStore, e: Expr, p: Pattern)
-      requires IsSafe(r,s,e,Type.String)
-      ensures IsSafe(r,s,UnaryApp(Like(p),e),Type.Bool(AnyBool))
-
-    lemma SetConstrSafe(r: Request, s: EntityStore, es: seq<Expr>, t: Type)
-      requires forall i :: 0 <= i < |es| ==> IsSafe(r,s,es[i],t)
-      ensures IsSafe(r,s,Expr.Set(es),Type.Set(t))
-
-    lemma ContainsAnyAllSafe(r: Request, s: EntityStore, op: BinaryOp, e1: Expr, e2: Expr, t1: Type, t2: Type)
-      requires op == ContainsAll || op == ContainsAny
-      requires IsSafe(r,s,e1,Type.Set(t1))
-      requires IsSafe(r,s,e2,Type.Set(t2))
-      ensures IsSafe(r,s,BinaryApp(op,e1,e2), Type.Bool(AnyBool))
-
-    lemma IneqSafe(r: Request, s: EntityStore, op: BinaryOp, e1: Expr, e2: Expr)
-      requires op == Less || op == BinaryOp.LessEq
-      requires IsSafe(r,s,e1,Type.Int)
-      requires IsSafe(r,s,e2,Type.Int)
-      ensures IsSafe(r,s,BinaryApp(op,e1,e2),Type.Bool(AnyBool))
-
-    lemma ArithSafe(r: Request, s: EntityStore, op: BinaryOp, e1: Expr, e2: Expr)
-      requires op == Add || op == Sub
-      requires IsSafe(r,s,e1,Type.Int)
-      requires IsSafe(r,s,e2,Type.Int)
-      ensures IsSafe(r,s,BinaryApp(op,e1,e2),Type.Int)
-
-    lemma CallSafe(r: Request, s: EntityStore, name: base.Name, args: seq<Expr>)
-      requires name in extFunTypes
-      requires |args| == |extFunTypes[name].args|
-      requires forall i | 0 <= i < |args| :: IsSafe(r,s,args[i],extFunTypes[name].args[i])
-      ensures IsSafe(r,s,Call(name,args),extFunTypes[name].ret)
-
-    lemma RecordSafe(r: Request, s: EntityStore, es: seq<(Attr,Expr)>, rt: RecordType)
-      //every entry has some type
-      requires forall ae :: ae in es ==> exists t :: IsSafe(r,s,ae.1,t)
-      //and the last instance of every required key is safe at the correct type.
-      requires forall k :: k in rt ==> KeyExists(k,es) && IsSafe(r,s,LastOfKey(k,es),rt[k].ty)
-      ensures IsSafe(r,s,Expr.Record(es),Type.Record(rt))
-
-    lemma ObjectProjSafeRequired(r: Request, s: EntityStore, e: Expr, t: Type, l: Attr, t': AttrType)
-      requires IsSafe(r,s,e,t)
-      requires SemanticSubty(t,Type.Record(map[l := t']))
-      requires t'.isRequired
-      ensures IsSafe(r,s,GetAttr(e,l),t'.ty)
-
-    lemma ObjectProjSafeGetAttrSafe(r: Request, s: EntityStore, e: Expr, t: Type, l: Attr, t': AttrType)
-      requires IsSafe(r,s,e,t)
-      requires SemanticSubty(t,Type.Record(map[l := t']))
-      requires GetAttrSafe(r,s,e,l)
-      ensures IsSafe(r,s,GetAttr(e,l),t'.ty)
-
-    ghost predicate ExistingEntityInLub(s: EntityStore, ev: EntityUID, lub: EntityLUB) {
-      InstanceOfType(Value.Primitive(Primitive.EntityUID(ev)),Type.Entity(lub)) && ev in s.entities
-    }
-
-    ghost predicate EntityProjStoreCondition(s: EntityStore, l: Attr, lub: EntityLUB, t': Type, isRequired: bool) {
-      forall ev: EntityUID | ExistingEntityInLub(s, ev, lub) ::
-        (isRequired ==> l in s.entities[ev].attrs) &&
-        (l in s.entities[ev].attrs ==> InstanceOfType(s.entities[ev].attrs[l],t'))
-    }
-
-    lemma EntityProjSafe(r: Request, s: EntityStore, e: Expr, l: Attr, lub: EntityLUB, t': Type, isRequired: bool)
-      requires IsSafe(r,s,e,Type.Entity(lub))
-      requires EntityProjStoreCondition(s, l, lub, t', isRequired)
-      requires isRequired || GetAttrSafe(r,s,e,l)
-      ensures IsSafe(r,s,GetAttr(e,l),t')
-
-    lemma RecordHasRequiredTrueSafe(r: Request, s: EntityStore, e: Expr, l: Attr, t: AttrType)
-      requires IsSafe(r,s,e,Type.Record(map[l := t]))
-      requires t.isRequired
-      ensures IsTrue(r,s,HasAttr(e,l))
-
-    lemma RecordHasOpenRecSafe(r: Request, s: EntityStore, e: Expr, l: Attr)
-      requires IsSafe(r,s,e,Type.Record(map[]))
-      ensures IsSafe(r,s,HasAttr(e,l),Type.Bool(AnyBool))
-
-    lemma EntityHasImpossibleFalseSafe(r: Request, s: EntityStore, e: Expr, l: Attr, lub: EntityLUB)
-      requires IsSafe(r,s,e,Type.Entity(lub))
-      requires forall ev: EntityUID | ExistingEntityInLub(s, ev, lub) ::
-                 l !in s.entities[ev].attrs
-      ensures IsFalse(r,s,HasAttr(e,l))
-
-    lemma EntityHasOpenSafe(r: Request, s: EntityStore, e: Expr, l: Attr)
-      requires IsSafe(r,s,e,Type.Entity(AnyEntity))
-      ensures IsSafe(r,s,HasAttr(e,l),Type.Bool(AnyBool))
-
-    lemma InSingleSafe(r: Request, s: EntityStore, e1: Expr, e2: Expr)
-      requires IsSafe(r,s,e1,Type.Entity(AnyEntity))
-      requires IsSafe(r,s,e2,Type.Entity(AnyEntity))
-      ensures IsSafe(r,s,BinaryApp(BinaryOp.In,e1,e2),Type.Bool(AnyBool))
-
-    // Duplicate Evaluator.EntityInEntity here so that SemanticModel and
-    // soundness.dfy don't have to depend on engine.dfy.
-    ghost predicate EntityInEntity(s: EntityStore, u1: EntityUID, u2: EntityUID) {
-      u1 == u2 || (s.getEntityAttrs(u1).Ok? && s.entityIn(u1, u2))
-    }
-
-    lemma InSingleFalseLiterals(r: Request, s: EntityStore, u1: EntityUID, u2: EntityUID)
-      requires !EntityInEntity(s,u1,u2)
-      ensures IsFalse(r,s,BinaryApp(BinaryOp.In,PrimitiveLit(Primitive.EntityUID(u1)),PrimitiveLit(Primitive.EntityUID(u2))))
-
-    lemma InSingleFalseEntityTypeAndLiteral(r: Request, s: EntityStore, e1: Expr, et1: EntityType, u2: EntityUID)
-      requires IsSafe(r,s,e1,Type.Entity(EntityLUB({et1})))
-      requires forall u1: EntityUID | u1.ty == et1 :: !EntityInEntity(s,u1,u2)
-      ensures IsFalse(r,s,BinaryApp(BinaryOp.In,e1,PrimitiveLit(Primitive.EntityUID(u2))))
-
-    lemma InSingleFalseTypes(r: Request, s: EntityStore, e1: Expr, e2: Expr, t1: Type, t2: Type)
-      requires subty(t1,Type.Entity(AnyEntity))
-      requires subty(t2,Type.Entity(AnyEntity))
-      requires IsSafe(r,s,e1,t1)
-      requires IsSafe(r,s,e2,t2)
-      requires forall u1, u2: EntityUID |
-        InstanceOfType(Value.EntityUID(u1), t1) && InstanceOfType(Value.EntityUID(u2), t2) ::
-        !EntityInEntity(s,u1,u2)
-      ensures IsFalse(r,s,BinaryApp(BinaryOp.In,e1,e2))
-
-    lemma InSetSafe(r: Request, s: EntityStore, e1: Expr, e2: Expr)
-      requires IsSafe(r,s,e1,Type.Entity(AnyEntity))
-      requires IsSafe(r,s,e2,Type.Set(Type.Entity(AnyEntity)))
-      ensures IsSafe(r,s,BinaryApp(BinaryOp.In,e1,e2),Type.Bool(AnyBool))
-
-    lemma InSetFalseIfAllFalse(r: Request, s: EntityStore, e1: Expr, e2s: seq<Expr>)
-      requires IsSafe(r,s,e1,Type.Entity(AnyEntity))
-      requires forall i | 0 <= i < |e2s| ::
-                 IsSafe(r,s,e2s[i],Type.Entity(AnyEntity)) &&
-                 IsFalse(r,s,BinaryApp(BinaryOp.In,e1,e2s[i]))
-      ensures IsFalse(r,s,BinaryApp(BinaryOp.In,e1,Expr.Set(e2s)))
-
-    lemma InSetFalseTypes(r: Request, s: EntityStore, e1: Expr, e2: Expr, t1: Type, t2: Type)
-      requires subty(t1,Type.Entity(AnyEntity))
-      requires subty(t2,Type.Entity(AnyEntity))
-      requires IsSafe(r,s,e1,t1)
-      requires IsSafe(r,s,e2,Type.Set(t2))
-      requires forall u1, u2: EntityUID |
-        InstanceOfType(Value.EntityUID(u1), t1) && InstanceOfType(Value.EntityUID(u2), t2) ::
-        !EntityInEntity(s,u1,u2)
-      ensures IsFalse(r,s,BinaryApp(BinaryOp.In,e1,e2))
+  ghost predicate IsTrue (r: Request, s: EntityStore, e: Expr) {
+    IsSafe(r,s,e,Type.Bool(True))
   }
 
-  // The particular model we're interested in is the EvaluatorModel, where a term
-  // is safe if it evaluates to a safe value or an error that is out-of-scope for
-  // the validator.
-  import opened def.engine
-  class EvaluatorModel extends SemanticModel {
-    ghost constructor(){}
+  ghost predicate IsFalse (r: Request, s: EntityStore, e: Expr) {
+    IsSafe(r,s,e,Type.Bool(False))
+  }
 
-    // An expression is safe if it evaluates to a value of the expected type
-    // or produces an error of type EntityDoesNotExist or ExtensionError.
-    //
-    // The validator cannot protect against errors where an entity literal is
-    // not defined in the entity store or extension errors, but it can protect
-    // against all other types of errors, namely: AttrDoesNotExist, TypeError,
-    // ArityMismatchError, NoSuchFunctionError
-    ghost predicate IsSafe(r: Request, s: EntityStore, e: Expr, t: Type) {
-      Evaluate(e,r,s) == base.Err(base.EntityDoesNotExist) ||
-      Evaluate(e,r,s) == base.Err(base.ExtensionError) ||
-      (Evaluate(e,r,s).Ok? && InstanceOfType(Evaluate(e,r,s).value,t))
+  ghost predicate GetAttrSafe (r: Request, s: EntityStore, e: Expr, k: Attr) {
+    IsTrue(r,s,HasAttr(e,k))
+  }
+
+  ghost predicate IsTrueStrong (r: Request, s: EntityStore, e: Expr) {
+    IsSafeStrong(r,s,e,Type.Bool(True))
+  }
+
+  ghost predicate IsFalseStrong (r: Request, s: EntityStore, e: Expr) {
+    IsSafeStrong(r,s,e,Type.Bool(False))
+  }
+
+  ghost predicate SemanticSubty(t1: Type, t2: Type) {
+    forall v :: InstanceOfType(v,t1) ==> InstanceOfType(v,t2)
+  }
+
+  ghost predicate SemanticUB(t1: Type, t2: Type, ub: Type) {
+    SemanticSubty(t1,ub) && SemanticSubty(t2,ub)
+  }
+
+  lemma SemSubtyTransportVal(t: Type, t': Type, v: Value)
+    requires SemanticSubty(t,t')
+    requires InstanceOfType(v,t)
+    ensures InstanceOfType(v,t')
+  {}
+
+  ghost predicate ExistingEntityInLub(s: EntityStore, ev: EntityUID, lub: EntityLUB) {
+    InstanceOfType(Value.Primitive(Primitive.EntityUID(ev)),Type.Entity(lub)) && ev in s.entities
+  }
+
+  ghost predicate EntityProjStoreCondition(s: EntityStore, l: Attr, lub: EntityLUB, t': Type, isRequired: bool) {
+    forall ev: EntityUID | ExistingEntityInLub(s, ev, lub) ::
+      (isRequired ==> l in s.entities[ev].attrs) &&
+      (l in s.entities[ev].attrs ==> InstanceOfType(s.entities[ev].attrs[l],t'))
+  }
+
+  // Duplicate Evaluator.EntityInEntity here so that SemanticModel and
+  // soundness.dfy don't have to depend on engine.dfy.
+  ghost predicate EntityInEntity(s: EntityStore, u1: EntityUID, u2: EntityUID) {
+    u1 == u2 || (s.getEntityAttrs(u1).Ok? && s.entityIn(u1, u2))
+  }
+
+  // An expression is safe if it evaluates to a value of the expected type
+  // or produces an error of type EntityDoesNotExist or ExtensionError.
+  //
+  // The validator cannot protect against errors where an entity literal is
+  // not defined in the entity store or extension errors, but it can protect
+  // against all other types of errors, namely: AttrDoesNotExist, TypeError,
+  // ArityMismatchError, NoSuchFunctionError
+  opaque ghost predicate IsSafe(r: Request, s: EntityStore, e: Expr, t: Type) {
+    Evaluate(e,r,s) == base.Err(base.EntityDoesNotExist) ||
+    Evaluate(e,r,s) == base.Err(base.ExtensionError) ||
+    (Evaluate(e,r,s).Ok? && InstanceOfType(Evaluate(e,r,s).value,t))
+  }
+
+  opaque ghost predicate IsSafeStrong (r: Request, s: EntityStore, e: Expr, t: Type) {
+    IsSafe(r,s,e,t) && Evaluate(e,r,s).Ok?
+  }
+
+  lemma IsTrueStrongImpliesIsTrue(r: Request, s: EntityStore, e: Expr)
+    requires IsTrueStrong(r,s,e)
+    ensures IsTrue(r,s,e)
+  {
+    reveal IsSafeStrong();
+  }
+
+  lemma IsTrueImpliesIsTrueStrong(r: Request, s: EntityStore, e: Expr, t: Type)
+    requires IsSafeStrong(r,s,e,t)
+    requires IsTrue(r,s,e)
+    ensures IsTrueStrong(r,s,e)
+  {
+    reveal IsSafeStrong();
+  }
+
+  lemma NotTrueImpliesFalse(r: Request, s: EntityStore, e: Expr, bt: BoolType)
+    requires IsSafe(r,s,e,Type.Bool(bt))
+    requires !IsTrue(r,s,e)
+    ensures IsFalse(r,s,e)
+  {
+    reveal IsSafe();
+  }
+
+  lemma NotSafeImpliesNotSafeStrong(r: Request, s: EntityStore, e: Expr, t: Type)
+    requires !IsSafe(r,s,e,t)
+    ensures !IsSafeStrong(r,s,e,t)
+  {
+    reveal IsSafeStrong();
+    reveal IsSafe();
+  }
+
+  lemma FalseImpliesNotTrueStrong(r: Request, s: EntityStore, e: Expr)
+    requires IsFalse(r,s,e)
+    ensures !IsTrueStrong(r,s,e)
+  {
+    reveal IsSafeStrong();
+    reveal IsSafe();
+  }
+
+  lemma SubtyCompat(t: Type, t': Type)
+    requires subty(t,t')
+    ensures SemanticSubty(t,t')
+  {
+    assert subty(t,t');
+    assert SemanticSubty(t,t') by {
+      forall v: Value | InstanceOfType(v,t)
+        ensures InstanceOfType(v,t')
+      {
+        SubtyCompatPointwise(t,t',v);
+      }
     }
+  }
 
-    ghost predicate IsSafeStrong (r: Request, s: EntityStore, e: Expr, t: Type) {
-      IsSafe(r,s,e,t) && Evaluate(e,r,s).Ok?
-    }
-
-    lemma IsTrueStrongImpliesIsTrue(r: Request, s: EntityStore, e: Expr)
-      requires IsTrueStrong(r,s,e)
-      ensures IsTrue(r,s,e)
-    {}
-
-    lemma IsTrueImpliesIsTrueStrong(r: Request, s: EntityStore, e: Expr, t: Type)
-      requires IsSafeStrong(r,s,e,t)
-      requires IsTrue(r,s,e)
-      ensures IsTrueStrong(r,s,e)
-    {}
-
-    lemma NotTrueImpliesFalse(r: Request, s: EntityStore, e: Expr, bt: BoolType)
-      requires IsSafe(r,s,e,Type.Bool(bt))
-      requires !IsTrue(r,s,e)
-      ensures IsFalse(r,s,e)
-    {}
-
-    lemma NotSafeImpliesNotSafeStrong(r: Request, s: EntityStore, e: Expr, t: Type)
-      requires !IsSafe(r,s,e,t)
-      ensures !IsSafeStrong(r,s,e,t)
-    {}
-
-    lemma FalseImpliesNotTrueStrong(r: Request, s: EntityStore, e: Expr)
-      requires IsFalse(r,s,e)
-      ensures !IsTrueStrong(r,s,e)
-    {}
-
-    lemma SubtyCompat(t: Type, t': Type)
-      requires subty(t,t')
-      ensures SemanticSubty(t,t')
-    {
-      assert subty(t,t');
-      assert SemanticSubty(t,t') by {
-        forall v: Value | InstanceOfType(v,t)
-          ensures InstanceOfType(v,t')
-        {
-          SubtyCompatPointwise(t,t',v);
+  lemma SubtyCompatMatchPointwise(t: Type, t': Type, v: Value)
+    requires subty(t,t')
+    requires InstanceOfType(v,t)
+    ensures InstanceOfType(v,t')
+    decreases t
+  {
+    match (t,t',v) {
+      case (Never,_,_) =>
+      case (String,String,_) =>
+      case (Int,Int,_) =>
+      case (Bool(b1),Bool(b2),_) =>
+      case (Set(t1),Set(t2),Set(s)) =>
+        assert forall v' | v' in s :: InstanceOfType(v',t2) by {
+          forall v': Value | v' in s
+            ensures InstanceOfType(v',t2)
+          {
+            assert InstanceOfType(v',t1);
+            SubtyCompatMatchPointwise(t1,t2,v');
+          }
         }
-      }
-    }
-
-    lemma SubtyCompatMatchPointwise(t: Type, t': Type, v: Value)
-      requires subty(t,t')
-      requires InstanceOfType(v,t)
-      ensures InstanceOfType(v,t')
-      decreases t
-    {
-      match (t,t',v) {
-        case (Never,_,_) =>
-        case (String,String,_) =>
-        case (Int,Int,_) =>
-        case (Bool(b1),Bool(b2),_) =>
-        case (Set(t1),Set(t2),Set(s)) =>
-          assert forall v' | v' in s :: InstanceOfType(v',t2) by {
-            forall v': Value | v' in s
-              ensures InstanceOfType(v',t2)
-            {
-              assert InstanceOfType(v',t1);
-              SubtyCompatMatchPointwise(t1,t2,v');
-            }
+      case (Record(rt1),Record(rt2),Record(rv)) =>
+        assert forall k | k in rt2 && k in rv :: InstanceOfType(rv[k],rt2[k].ty) by {
+          forall k: Attr | k in rt2 && k in rv
+            ensures InstanceOfType(rv[k],rt2[k].ty)
+          {
+            assert InstanceOfType(rv[k],rt1[k].ty);
+            assert subtyAttrType(rt1[k],rt2[k]);
+            SubtyCompatMatchPointwise(rt1[k].ty,rt2[k].ty,rv[k]);
           }
-        case (Record(rt1),Record(rt2),Record(rv)) =>
-          assert forall k | k in rt2 && k in rv :: InstanceOfType(rv[k],rt2[k].ty) by {
-            forall k: Attr | k in rt2 && k in rv
-              ensures InstanceOfType(rv[k],rt2[k].ty)
-            {
-              assert InstanceOfType(rv[k],rt1[k].ty);
-              assert subtyAttrType(rt1[k],rt2[k]);
-              SubtyCompatMatchPointwise(rt1[k].ty,rt2[k].ty,rv[k]);
-            }
-          }
-          assert forall k | k in rt2 && rt2[k].isRequired :: k in rv by {
-            forall k | k in rt2 && rt2[k].isRequired
-              ensures k in rv
-            {
-              assert subtyAttrType(rt1[k],rt2[k]);
-            }
-          }
-        case (Entity(e1),Entity(e2),_) =>
-        case (Extension(e1),Extension(e2),_) =>
-      }
-    }
-
-    lemma SubtyCompatPointwise(t: Type, t': Type, v: Value)
-      requires subty(t,t')
-      requires InstanceOfType(v,t)
-      ensures InstanceOfType(v,t')
-    {
-      SubtyCompatMatchPointwise(t,t',v);
-    }
-
-    lemma SemSubtyTransport(r: Request, s: EntityStore, e: Expr, t: Type, t': Type)
-      requires SemanticSubty(t,t')
-      requires IsSafe(r,s,e,t)
-      ensures IsSafe(r,s,e,t')
-    {
-      if (exists v :: Evaluate(e,r,s) == base.Ok(v) && InstanceOfType(v,t)) {
-        var v :| Evaluate(e,r,s) == base.Ok(v) && InstanceOfType(v,t);
-        assert InstanceOfType(v,t') by {
-          SemSubtyTransportVal(t,t',v);
         }
+        assert forall k | k in rt2 && rt2[k].isRequired :: k in rv by {
+          forall k | k in rt2 && rt2[k].isRequired
+            ensures k in rv
+          {
+            assert subtyAttrType(rt1[k],rt2[k]);
+          }
+        }
+      case (Entity(e1),Entity(e2),_) =>
+      case (Extension(e1),Extension(e2),_) =>
+    }
+  }
+
+  lemma SubtyCompatPointwise(t: Type, t': Type, v: Value)
+    requires subty(t,t')
+    requires InstanceOfType(v,t)
+    ensures InstanceOfType(v,t')
+  {
+    SubtyCompatMatchPointwise(t,t',v);
+  }
+
+  lemma SemSubtyTransport(r: Request, s: EntityStore, e: Expr, t: Type, t': Type)
+    requires SemanticSubty(t,t')
+    requires IsSafe(r,s,e,t)
+    ensures IsSafe(r,s,e,t')
+  {
+    reveal IsSafe();
+    if (exists v :: Evaluate(e,r,s) == base.Ok(v) && InstanceOfType(v,t)) {
+      var v :| Evaluate(e,r,s) == base.Ok(v) && InstanceOfType(v,t);
+      assert InstanceOfType(v,t') by {
+        SemSubtyTransportVal(t,t',v);
       }
     }
+  }
 
-    lemma PrincipalIsSafe(r: Request, s: EntityStore, t: Type)
-      requires InstanceOfType(Value.EntityUID(r.principal),t)
-      ensures IsSafe(r,s,Var(Principal),t)
-    {}
+  lemma PrincipalIsSafe(r: Request, s: EntityStore, t: Type)
+    requires InstanceOfType(Value.EntityUID(r.principal),t)
+    ensures IsSafe(r,s,Var(Principal),t)
+  {
+    reveal IsSafe();
+  }
 
-    lemma ActionIsSafe(r: Request, s: EntityStore, t: Type)
-      requires InstanceOfType(Value.EntityUID(r.action),t)
-      ensures IsSafe(r,s,Var(Action),t)
-    {}
+  lemma ActionIsSafe(r: Request, s: EntityStore, t: Type)
+    requires InstanceOfType(Value.EntityUID(r.action),t)
+    ensures IsSafe(r,s,Var(Action),t)
+  {
+    reveal IsSafe();
+  }
 
-    lemma ResourceIsSafe(r: Request, s: EntityStore, t: Type)
-      requires InstanceOfType(Value.EntityUID(r.resource),t)
-      ensures IsSafe(r,s,Var(Resource),t)
-    {}
+  lemma ResourceIsSafe(r: Request, s: EntityStore, t: Type)
+    requires InstanceOfType(Value.EntityUID(r.resource),t)
+    ensures IsSafe(r,s,Var(Resource),t)
+  {
+    reveal IsSafe();
+  }
 
-    lemma ContextIsSafe(r: Request, s: EntityStore, t: Type)
-      requires InstanceOfType(Value.Record(r.context),t)
-      ensures IsSafe(r,s,Var(Context),t)
-    {}
+  lemma ContextIsSafe(r: Request, s: EntityStore, t: Type)
+    requires InstanceOfType(Value.Record(r.context),t)
+    ensures IsSafe(r,s,Var(Context),t)
+  {
+    reveal IsSafe();
+  }
 
-    lemma PrimSafeLift(r: Request, s: EntityStore, p: Primitive, t: Type)
-      requires InstanceOfType(Value.Primitive(p),t)
-      ensures IsSafe(r,s,Expr.PrimitiveLit(p),t)
-    {}
+  lemma PrimSafeLift(r: Request, s: EntityStore, p: Primitive, t: Type)
+    requires InstanceOfType(Value.Primitive(p),t)
+    ensures IsSafe(r,s,Expr.PrimitiveLit(p),t)
+  {
+    reveal IsSafe();
+  }
 
-    lemma PrimSafeAtInferredType(p: Primitive)
-      ensures InstanceOfType(Value.Primitive(p),typeOfPrim(p))
-    {}
+  lemma PrimSafeAtInferredType(p: Primitive)
+    ensures InstanceOfType(Value.Primitive(p),typeOfPrim(p))
+  {}
 
-    lemma EqIsSafe(r: Request, s: EntityStore, e: Expr, e': Expr, t: Type, t': Type)
-      requires IsSafe(r,s,e,t)
-      requires IsSafe(r,s,e',t')
-      ensures IsSafe(r,s,BinaryApp(BinaryOp.Eq,e,e'),Type.Bool(AnyBool))
-    {}
+  lemma EqIsSafe(r: Request, s: EntityStore, e: Expr, e': Expr, t: Type, t': Type)
+    requires IsSafe(r,s,e,t)
+    requires IsSafe(r,s,e',t')
+    ensures IsSafe(r,s,BinaryApp(BinaryOp.Eq,e,e'),Type.Bool(AnyBool))
+  {
+    reveal IsSafe();
+  }
 
-    lemma EqFalseIsSafe(r: Request, s: EntityStore, e: Expr, e': Expr, lub: EntityLUB, lub': EntityLUB)
-      requires IsSafe(r,s,e,Type.Entity(lub))
-      requires IsSafe(r,s,e',Type.Entity(lub'))
-      requires lub.disjoint(lub')
-      ensures IsFalse(r,s,BinaryApp(BinaryOp.Eq,e,e'))
-    {}
+  lemma EqFalseIsSafe(r: Request, s: EntityStore, e: Expr, e': Expr, lub: EntityLUB, lub': EntityLUB)
+    requires IsSafe(r,s,e,Type.Entity(lub))
+    requires IsSafe(r,s,e',Type.Entity(lub'))
+    requires lub.disjoint(lub')
+    ensures IsFalse(r,s,BinaryApp(BinaryOp.Eq,e,e'))
+  {
+    reveal IsSafe();
+  }
 
-    lemma EqEntitySameSafe(r: Request, s: EntityStore, E: EntityUID)
-      ensures IsTrue(r,s,Expr.BinaryApp(BinaryOp.Eq,PrimitiveLit(Primitive.EntityUID(E)),PrimitiveLit(Primitive.EntityUID(E))))
-    {
-      var e := Expr.BinaryApp(BinaryOp.Eq,PrimitiveLit(Primitive.EntityUID(E)),PrimitiveLit(Primitive.EntityUID(E)));
-      assert Evaluator(r,s).interpret(e) == base.Ok(Value.Primitive(Primitive.Bool(true)));
+  lemma EqEntitySameSafe(r: Request, s: EntityStore, E: EntityUID)
+    ensures IsTrue(r,s,Expr.BinaryApp(BinaryOp.Eq,PrimitiveLit(Primitive.EntityUID(E)),PrimitiveLit(Primitive.EntityUID(E))))
+  {
+    reveal IsSafe();
+    var e := Expr.BinaryApp(BinaryOp.Eq,PrimitiveLit(Primitive.EntityUID(E)),PrimitiveLit(Primitive.EntityUID(E)));
+    assert Evaluator(r,s).interpret(e) == base.Ok(Value.Primitive(Primitive.Bool(true)));
+  }
+
+  lemma EqEntityDiffSafe(r: Request, s: EntityStore, E: EntityUID, E': EntityUID)
+    requires E != E'
+    ensures IsFalse(r,s,Expr.BinaryApp(BinaryOp.Eq,PrimitiveLit(Primitive.EntityUID(E)),PrimitiveLit(Primitive.EntityUID(E'))))
+  {
+    reveal IsSafe();
+    var e := Expr.BinaryApp(BinaryOp.Eq,PrimitiveLit(Primitive.EntityUID(E)),PrimitiveLit(Primitive.EntityUID(E')));
+    assert Evaluator(r,s).interpret(e) == base.Ok(Value.Primitive(Primitive.Bool(false)));
+  }
+
+  lemma AndLShortSafe(r: Request, s: EntityStore, e: Expr, e': Expr)
+    requires IsFalse(r,s,e)
+    ensures IsFalse(r,s,And(e,e'))
+  {
+    reveal IsSafe();
+    if Evaluate(e,r,s).Ok? {
+      assert Evaluate(e,r,s) == base.Ok(Value.Primitive(Primitive.Bool(false)));
+      assert Evaluator(r,s).interpretShortcircuit(And(e,e'),e,e',false) == base.Ok(Value.Primitive(Primitive.Bool(false)));
+      assert Evaluate(And(e,e'),r,s) == base.Ok(Value.Primitive(Primitive.Bool(false)));
+    } else {
+      assert Evaluator(r,s).interpretShortcircuit(And(e,e'),e,e',false) == Evaluate(e,r,s);
+      assert Evaluate(And(e,e'),r,s) == Evaluate(e,r,s);
     }
+  }
 
-    lemma EqEntityDiffSafe(r: Request, s: EntityStore, E: EntityUID, E': EntityUID)
-      requires E != E'
-      ensures IsFalse(r,s,Expr.BinaryApp(BinaryOp.Eq,PrimitiveLit(Primitive.EntityUID(E)),PrimitiveLit(Primitive.EntityUID(E'))))
-    {
-      var e := Expr.BinaryApp(BinaryOp.Eq,PrimitiveLit(Primitive.EntityUID(E)),PrimitiveLit(Primitive.EntityUID(E')));
-      assert Evaluator(r,s).interpret(e) == base.Ok(Value.Primitive(Primitive.Bool(false)));
-    }
-
-    lemma AndLShortSafe(r: Request, s: EntityStore, e: Expr, e': Expr)
-      requires IsFalse(r,s,e)
-      ensures IsFalse(r,s,And(e,e'))
-    {
-      if Evaluate(e,r,s).Ok? {
-        assert Evaluate(e,r,s) == base.Ok(Value.Primitive(Primitive.Bool(false)));
-        assert Evaluator(r,s).interpretShortcircuit(And(e,e'),e,e',false) == base.Ok(Value.Primitive(Primitive.Bool(false)));
-        assert Evaluate(And(e,e'),r,s) == base.Ok(Value.Primitive(Primitive.Bool(false)));
-      } else {
+  lemma AndRShortSafe(r: Request, s: EntityStore, e: Expr, e': Expr)
+    requires IsSafe(r,s,e,Type.Bool(AnyBool))
+    requires IsFalse(r,s,e')
+    ensures IsFalse(r,s,And(e,e'))
+  {
+    reveal IsSafe();
+    if Evaluate(e,r,s).Ok? && Evaluate(e',r,s).Ok? {
+      assert Evaluate(e',r,s) == base.Ok(Value.Primitive(Primitive.Bool(false)));
+      assert Evaluator(r,s).interpretShortcircuit(And(e,e'),e,e',false) == base.Ok(Value.Primitive(Primitive.Bool(false)));
+      assert Evaluate(And(e,e'),r,s) == base.Ok(Value.Primitive(Primitive.Bool(false)));
+    } else {
+      if Evaluate(e,r,s).Err? {
         assert Evaluator(r,s).interpretShortcircuit(And(e,e'),e,e',false) == Evaluate(e,r,s);
         assert Evaluate(And(e,e'),r,s) == Evaluate(e,r,s);
-      }
-    }
-
-    lemma AndRShortSafe(r: Request, s: EntityStore, e: Expr, e': Expr)
-      requires IsSafe(r,s,e,Type.Bool(AnyBool))
-      requires IsFalse(r,s,e')
-      ensures IsFalse(r,s,And(e,e'))
-    {
-      if Evaluate(e,r,s).Ok? && Evaluate(e',r,s).Ok? {
-        assert Evaluate(e',r,s) == base.Ok(Value.Primitive(Primitive.Bool(false)));
-        assert Evaluator(r,s).interpretShortcircuit(And(e,e'),e,e',false) == base.Ok(Value.Primitive(Primitive.Bool(false)));
-        assert Evaluate(And(e,e'),r,s) == base.Ok(Value.Primitive(Primitive.Bool(false)));
       } else {
-        if Evaluate(e,r,s).Err? {
-          assert Evaluator(r,s).interpretShortcircuit(And(e,e'),e,e',false) == Evaluate(e,r,s);
-          assert Evaluate(And(e,e'),r,s) == Evaluate(e,r,s);
+        assert Evaluate(e',r,s).Err?;
+        var b :| Evaluate(e,r,s) == base.Ok(Value.Primitive(Primitive.Bool(b)));
+        if b {
+          assert Evaluator(r,s).interpretShortcircuit(And(e,e'),e,e',false) == Evaluate(e',r,s);
+          assert Evaluate(And(e,e'),r,s) == Evaluate(e',r,s);
         } else {
-          assert Evaluate(e',r,s).Err?;
-          var b :| Evaluate(e,r,s) == base.Ok(Value.Primitive(Primitive.Bool(b)));
-          if b {
-            assert Evaluator(r,s).interpretShortcircuit(And(e,e'),e,e',false) == Evaluate(e',r,s);
-            assert Evaluate(And(e,e'),r,s) == Evaluate(e',r,s);
-          } else {
-            assert Evaluator(r,s).interpretShortcircuit(And(e,e'),e,e',false) == base.Ok(Value.Primitive(Primitive.Bool(false)));
-            assert Evaluate(And(e,e'),r,s) == base.Ok(Value.Primitive(Primitive.Bool(false)));
-          }
+          assert Evaluator(r,s).interpretShortcircuit(And(e,e'),e,e',false) == base.Ok(Value.Primitive(Primitive.Bool(false)));
+          assert Evaluate(And(e,e'),r,s) == base.Ok(Value.Primitive(Primitive.Bool(false)));
         }
       }
     }
+  }
 
-    lemma AndLRetSafe(r: Request, s: EntityStore, e: Expr, e': Expr, t: Type)
-      requires IsSafe(r,s,e,t)
-      requires IsTrue(r,s,e')
-      requires SemanticSubty(t,Type.Bool(AnyBool))
-      ensures IsSafe(r,s,And(e,e'),t)
-    {
-      if Evaluate(e,r,s).Ok? && Evaluate(e',r,s).Ok? {
-        assert Evaluate(e',r,s) == base.Ok(Value.Primitive(Primitive.Bool(true)));
-        var v :| Evaluate(e,r,s) == base.Ok(v) && InstanceOfType(v,t);
-        assert InstanceOfType(v,Type.Bool(AnyBool)) by {
-          SemSubtyTransportVal(t,Type.Bool(AnyBool),v);
-        }
-        var b :| v == Value.Primitive(Primitive.Bool(b));
-        assert Evaluator(r,s).interpretShortcircuit(And(e,e'),e,e',false) == base.Ok(Value.Primitive(Primitive.Bool(b)));
-        assert Evaluate(And(e,e'),r,s) == base.Ok(Value.Primitive(Primitive.Bool(b)));
+  lemma AndLRetSafe(r: Request, s: EntityStore, e: Expr, e': Expr, t: Type)
+    requires IsSafe(r,s,e,t)
+    requires IsTrue(r,s,e')
+    requires SemanticSubty(t,Type.Bool(AnyBool))
+    ensures IsSafe(r,s,And(e,e'),t)
+  {
+    reveal IsSafe();
+    if Evaluate(e,r,s).Ok? && Evaluate(e',r,s).Ok? {
+      assert Evaluate(e',r,s) == base.Ok(Value.Primitive(Primitive.Bool(true)));
+      var v :| Evaluate(e,r,s) == base.Ok(v) && InstanceOfType(v,t);
+      assert InstanceOfType(v,Type.Bool(AnyBool)) by {
+        SemSubtyTransportVal(t,Type.Bool(AnyBool),v);
+      }
+      var b :| v == Value.Primitive(Primitive.Bool(b));
+      assert Evaluator(r,s).interpretShortcircuit(And(e,e'),e,e',false) == base.Ok(Value.Primitive(Primitive.Bool(b)));
+      assert Evaluate(And(e,e'),r,s) == base.Ok(Value.Primitive(Primitive.Bool(b)));
+    } else {
+      if Evaluate(e,r,s).Err? {
+        assert Evaluator(r,s).interpretShortcircuit(And(e,e'),e,e',false) == Evaluate(e,r,s);
+        assert Evaluate(And(e,e'),r,s) == Evaluate(e,r,s);
       } else {
-        if Evaluate(e,r,s).Err? {
-          assert Evaluator(r,s).interpretShortcircuit(And(e,e'),e,e',false) == Evaluate(e,r,s);
-          assert Evaluate(And(e,e'),r,s) == Evaluate(e,r,s);
+        assert Evaluate(e',r,s).Err?;
+        var b :| Evaluate(e,r,s) == base.Ok(Value.Primitive(Primitive.Bool(b)));
+        if b {
+          assert Evaluator(r,s).interpretShortcircuit(And(e,e'),e,e',false) == Evaluate(e',r,s);
+          assert Evaluate(And(e,e'),r,s) == Evaluate(e',r,s);
         } else {
-          assert Evaluate(e',r,s).Err?;
-          var b :| Evaluate(e,r,s) == base.Ok(Value.Primitive(Primitive.Bool(b)));
-          if b {
-            assert Evaluator(r,s).interpretShortcircuit(And(e,e'),e,e',false) == Evaluate(e',r,s);
-            assert Evaluate(And(e,e'),r,s) == Evaluate(e',r,s);
-          } else {
-            assert Evaluator(r,s).interpretShortcircuit(And(e,e'),e,e',false) == base.Ok(Value.Primitive(Primitive.Bool(false)));
-            assert Evaluate(And(e,e'),r,s) == base.Ok(Value.Primitive(Primitive.Bool(false)));
-          }
+          assert Evaluator(r,s).interpretShortcircuit(And(e,e'),e,e',false) == base.Ok(Value.Primitive(Primitive.Bool(false)));
+          assert Evaluate(And(e,e'),r,s) == base.Ok(Value.Primitive(Primitive.Bool(false)));
         }
       }
     }
+  }
 
-    lemma AndSafe(r: Request, s: EntityStore, e: Expr, e': Expr)
-      requires IsSafe(r,s,e,Type.Bool(AnyBool))
-      requires IsSafe(r,s,e',Type.Bool(AnyBool))
-      ensures IsSafe(r,s,And(e,e'),Type.Bool(AnyBool))
-    {
-      if Evaluate(e,r,s).Ok? && Evaluate(e',r,s).Ok? {
-        assert Evaluator(r,s).interpretShortcircuit(And(e,e'),e,e',false).Ok?;
-        assert Evaluate(And(e,e'),r,s).Ok?;
+  lemma AndSafe(r: Request, s: EntityStore, e: Expr, e': Expr)
+    requires IsSafe(r,s,e,Type.Bool(AnyBool))
+    requires IsSafe(r,s,e',Type.Bool(AnyBool))
+    ensures IsSafe(r,s,And(e,e'),Type.Bool(AnyBool))
+  {
+    reveal IsSafe();
+    if Evaluate(e,r,s).Ok? && Evaluate(e',r,s).Ok? {
+      assert Evaluator(r,s).interpretShortcircuit(And(e,e'),e,e',false).Ok?;
+      assert Evaluate(And(e,e'),r,s).Ok?;
+    } else {
+      if Evaluate(e,r,s).Err? {
+        assert Evaluator(r,s).interpretShortcircuit(And(e,e'),e,e',false) == Evaluate(e,r,s);
+        assert Evaluate(And(e,e'),r,s) == Evaluate(e,r,s);
       } else {
-        if Evaluate(e,r,s).Err? {
-          assert Evaluator(r,s).interpretShortcircuit(And(e,e'),e,e',false) == Evaluate(e,r,s);
-          assert Evaluate(And(e,e'),r,s) == Evaluate(e,r,s);
+        assert Evaluate(e',r,s).Err?;
+        var b :| Evaluate(e,r,s) == base.Ok(Value.Primitive(Primitive.Bool(b)));
+        if b {
+          assert Evaluator(r,s).interpretShortcircuit(And(e,e'),e,e',false) == Evaluate(e',r,s);
+          assert Evaluate(And(e,e'),r,s) == Evaluate(e',r,s);
         } else {
-          assert Evaluate(e',r,s).Err?;
-          var b :| Evaluate(e,r,s) == base.Ok(Value.Primitive(Primitive.Bool(b)));
-          if b {
-            assert Evaluator(r,s).interpretShortcircuit(And(e,e'),e,e',false) == Evaluate(e',r,s);
-            assert Evaluate(And(e,e'),r,s) == Evaluate(e',r,s);
-          } else {
-            assert Evaluator(r,s).interpretShortcircuit(And(e,e'),e,e',false) == base.Ok(Value.Primitive(Primitive.Bool(false)));
-            assert Evaluate(And(e,e'),r,s) == base.Ok(Value.Primitive(Primitive.Bool(false)));
-          }
+          assert Evaluator(r,s).interpretShortcircuit(And(e,e'),e,e',false) == base.Ok(Value.Primitive(Primitive.Bool(false)));
+          assert Evaluate(And(e,e'),r,s) == base.Ok(Value.Primitive(Primitive.Bool(false)));
         }
       }
     }
+  }
 
-    lemma AndTrueStrong(r: Request, s: EntityStore, e1: Expr, e2: Expr)
-      requires IsTrue(r,s,e1)
-      requires IsTrueStrong(r,s,And(e1,e2))
-      ensures IsTrueStrong(r,s,e2)
-    {
-      assert Evaluator(r,s).interpretShortcircuit(And(e1,e2),e1,e2,false) == base.Ok(Value.Bool(true));
+  lemma AndTrueStrong(r: Request, s: EntityStore, e1: Expr, e2: Expr)
+    requires IsTrue(r,s,e1)
+    requires IsTrueStrong(r,s,And(e1,e2))
+    ensures IsTrueStrong(r,s,e2)
+  {
+    reveal IsSafeStrong();
+    reveal IsSafe();
+    assert Evaluator(r,s).interpretShortcircuit(And(e1,e2),e1,e2,false) == base.Ok(Value.Bool(true));
+  }
+
+  lemma AndError(r: Request, s: EntityStore, e1: Expr, e2: Expr, t: Type, tnew: Type)
+    requires IsSafe(r,s,e1,t)
+    requires !IsSafeStrong(r,s,e1,t)
+    ensures IsSafe(r,s,And(e1,e2),tnew)
+    ensures !IsSafeStrong(r,s,And(e1,e2),tnew)
+  {
+    reveal IsSafeStrong();
+    reveal IsSafe();
+    assert Evaluator(r,s).interpretShortcircuit(And(e1,e2),e1,e2,false).Err?;
+  }
+
+  lemma OrLShortSafe(r: Request, s: EntityStore, e: Expr, e': Expr)
+    requires IsTrue(r,s,e)
+    ensures IsTrue(r,s,Or(e,e'))
+  {
+    reveal IsSafe();
+    if Evaluate(e,r,s).Ok? {
+      assert Evaluate(e,r,s) == base.Ok(Value.Primitive(Primitive.Bool(true)));
+      assert Evaluator(r,s).interpretShortcircuit(Or(e,e'),e,e',true) == base.Ok(Value.Primitive(Primitive.Bool(true)));
+      assert Evaluate(Or(e,e'),r,s) == base.Ok(Value.Primitive(Primitive.Bool(true)));
+    } else {
+      assert Evaluator(r,s).interpretShortcircuit(Or(e,e'),e,e',true) == Evaluate(e,r,s);
+      assert Evaluate(Or(e,e'),r,s) == Evaluate(e,r,s);
     }
+  }
 
-    lemma AndError(r: Request, s: EntityStore, e1: Expr, e2: Expr, t: Type, tnew: Type)
-      requires IsSafe(r,s,e1,t)
-      requires !IsSafeStrong(r,s,e1,t)
-      ensures IsSafe(r,s,And(e1,e2),tnew)
-      ensures !IsSafeStrong(r,s,And(e1,e2),tnew)
-    {
-      assert Evaluator(r,s).interpretShortcircuit(And(e1,e2),e1,e2,false).Err?;
-    }
-
-    lemma OrLShortSafe(r: Request, s: EntityStore, e: Expr, e': Expr)
-      requires IsTrue(r,s,e)
-      ensures IsTrue(r,s,Or(e,e'))
-    {
-      if Evaluate(e,r,s).Ok? {
-        assert Evaluate(e,r,s) == base.Ok(Value.Primitive(Primitive.Bool(true)));
-        assert Evaluator(r,s).interpretShortcircuit(Or(e,e'),e,e',true) == base.Ok(Value.Primitive(Primitive.Bool(true)));
-        assert Evaluate(Or(e,e'),r,s) == base.Ok(Value.Primitive(Primitive.Bool(true)));
-      } else {
+  lemma OrRShortSafe(r: Request, s: EntityStore, e: Expr, e': Expr)
+    requires IsSafe(r,s,e,Type.Bool(AnyBool))
+    requires IsTrue(r,s,e')
+    ensures IsTrue(r,s,Or(e,e'))
+  {
+    reveal IsSafe();
+    if Evaluate(e,r,s).Ok? && Evaluate(e',r,s).Ok? {
+      assert Evaluate(e',r,s) == base.Ok(Value.Primitive(Primitive.Bool(true)));
+      assert Evaluator(r,s).interpretShortcircuit(Or(e,e'),e,e',true) == base.Ok(Value.Primitive(Primitive.Bool(true)));
+      assert Evaluate(Or(e,e'),r,s) == base.Ok(Value.Primitive(Primitive.Bool(true)));
+    } else {
+      if Evaluate(e,r,s).Err? {
         assert Evaluator(r,s).interpretShortcircuit(Or(e,e'),e,e',true) == Evaluate(e,r,s);
         assert Evaluate(Or(e,e'),r,s) == Evaluate(e,r,s);
-      }
-    }
-
-    lemma OrRShortSafe(r: Request, s: EntityStore, e: Expr, e': Expr)
-      requires IsSafe(r,s,e,Type.Bool(AnyBool))
-      requires IsTrue(r,s,e')
-      ensures IsTrue(r,s,Or(e,e'))
-    {
-      if Evaluate(e,r,s).Ok? && Evaluate(e',r,s).Ok? {
-        assert Evaluate(e',r,s) == base.Ok(Value.Primitive(Primitive.Bool(true)));
-        assert Evaluator(r,s).interpretShortcircuit(Or(e,e'),e,e',true) == base.Ok(Value.Primitive(Primitive.Bool(true)));
-        assert Evaluate(Or(e,e'),r,s) == base.Ok(Value.Primitive(Primitive.Bool(true)));
       } else {
-        if Evaluate(e,r,s).Err? {
-          assert Evaluator(r,s).interpretShortcircuit(Or(e,e'),e,e',true) == Evaluate(e,r,s);
-          assert Evaluate(Or(e,e'),r,s) == Evaluate(e,r,s);
+        assert Evaluate(e',r,s).Err?;
+        var b :| Evaluate(e,r,s) == base.Ok(Value.Primitive(Primitive.Bool(b)));
+        if b {
+          assert Evaluator(r,s).interpretShortcircuit(Or(e,e'),e,e',true) == base.Ok(Value.Primitive(Primitive.Bool(true)));
+          assert Evaluate(Or(e,e'),r,s) == base.Ok(Value.Primitive(Primitive.Bool(true)));
         } else {
-          assert Evaluate(e',r,s).Err?;
-          var b :| Evaluate(e,r,s) == base.Ok(Value.Primitive(Primitive.Bool(b)));
-          if b {
-            assert Evaluator(r,s).interpretShortcircuit(Or(e,e'),e,e',true) == base.Ok(Value.Primitive(Primitive.Bool(true)));
-            assert Evaluate(Or(e,e'),r,s) == base.Ok(Value.Primitive(Primitive.Bool(true)));
-          } else {
-            assert Evaluator(r,s).interpretShortcircuit(Or(e,e'),e,e',true) == Evaluate(e',r,s);
-            assert Evaluate(Or(e,e'),r,s) == Evaluate(e',r,s);
-          }
+          assert Evaluator(r,s).interpretShortcircuit(Or(e,e'),e,e',true) == Evaluate(e',r,s);
+          assert Evaluate(Or(e,e'),r,s) == Evaluate(e',r,s);
         }
       }
     }
+  }
 
-    lemma OrLRetSafe(r: Request, s: EntityStore, e: Expr, e': Expr, t: Type)
-      requires IsSafe(r,s,e,t)
-      requires IsFalse(r,s,e')
-      requires SemanticSubty(t,Type.Bool(AnyBool))
-      ensures IsSafe(r,s,Or(e,e'),t)
-    {
-      if Evaluate(e,r,s).Ok? && Evaluate(e',r,s).Ok? {
-        assert Evaluate(e',r,s) == base.Ok(Value.Primitive(Primitive.Bool(false)));
-        var v :| Evaluate(e,r,s) == base.Ok(v) && InstanceOfType(v,t);
-        assert InstanceOfType(v,Type.Bool(AnyBool)) by {
-          SemSubtyTransportVal(t,Type.Bool(AnyBool),v);
-        }
-        var b :| v == Value.Primitive(Primitive.Bool(b));
-        assert Evaluator(r,s).interpretShortcircuit(Or(e,e'),e,e',true) == base.Ok(Value.Primitive(Primitive.Bool(b)));
-        assert Evaluate(Or(e,e'),r,s) == base.Ok(Value.Primitive(Primitive.Bool(b)));
-        assert IsSafe(r,s,e,Type.Bool(AnyBool)) by {
-          SemSubtyTransport(r,s,e,t,Type.Bool(AnyBool));
-        }
+  lemma OrLRetSafe(r: Request, s: EntityStore, e: Expr, e': Expr, t: Type)
+    requires IsSafe(r,s,e,t)
+    requires IsFalse(r,s,e')
+    requires SemanticSubty(t,Type.Bool(AnyBool))
+    ensures IsSafe(r,s,Or(e,e'),t)
+  {
+    reveal IsSafe();
+    if Evaluate(e,r,s).Ok? && Evaluate(e',r,s).Ok? {
+      assert Evaluate(e',r,s) == base.Ok(Value.Primitive(Primitive.Bool(false)));
+      var v :| Evaluate(e,r,s) == base.Ok(v) && InstanceOfType(v,t);
+      assert InstanceOfType(v,Type.Bool(AnyBool)) by {
+        SemSubtyTransportVal(t,Type.Bool(AnyBool),v);
+      }
+      var b :| v == Value.Primitive(Primitive.Bool(b));
+      assert Evaluator(r,s).interpretShortcircuit(Or(e,e'),e,e',true) == base.Ok(Value.Primitive(Primitive.Bool(b)));
+      assert Evaluate(Or(e,e'),r,s) == base.Ok(Value.Primitive(Primitive.Bool(b)));
+      assert IsSafe(r,s,e,Type.Bool(AnyBool)) by {
+        SemSubtyTransport(r,s,e,t,Type.Bool(AnyBool));
+      }
+    } else {
+      if Evaluate(e,r,s).Err? {
+        assert Evaluator(r,s).interpretShortcircuit(Or(e,e'),e,e',true) == Evaluate(e,r,s);
+        assert Evaluate(Or(e,e'),r,s) == Evaluate(e,r,s);
       } else {
-        if Evaluate(e,r,s).Err? {
-          assert Evaluator(r,s).interpretShortcircuit(Or(e,e'),e,e',true) == Evaluate(e,r,s);
-          assert Evaluate(Or(e,e'),r,s) == Evaluate(e,r,s);
+        assert Evaluate(e',r,s).Err?;
+        var b :| Evaluate(e,r,s) == base.Ok(Value.Primitive(Primitive.Bool(b)));
+        if b {
+          assert Evaluator(r,s).interpretShortcircuit(Or(e,e'),e,e',true) == base.Ok(Value.Primitive(Primitive.Bool(true)));
+          assert Evaluate(Or(e,e'),r,s) == base.Ok(Value.Primitive(Primitive.Bool(true)));
         } else {
-          assert Evaluate(e',r,s).Err?;
-          var b :| Evaluate(e,r,s) == base.Ok(Value.Primitive(Primitive.Bool(b)));
-          if b {
-            assert Evaluator(r,s).interpretShortcircuit(Or(e,e'),e,e',true) == base.Ok(Value.Primitive(Primitive.Bool(true)));
-            assert Evaluate(Or(e,e'),r,s) == base.Ok(Value.Primitive(Primitive.Bool(true)));
-          } else {
-            assert Evaluator(r,s).interpretShortcircuit(Or(e,e'),e,e',true) == Evaluate(e',r,s);
-            assert Evaluate(Or(e,e'),r,s) == Evaluate(e',r,s);
-          }
+          assert Evaluator(r,s).interpretShortcircuit(Or(e,e'),e,e',true) == Evaluate(e',r,s);
+          assert Evaluate(Or(e,e'),r,s) == Evaluate(e',r,s);
         }
       }
     }
+  }
 
-    lemma OrRRetSafe(r: Request, s: EntityStore, e: Expr, e': Expr, t: Type)
-      requires IsFalse(r,s,e)
-      requires IsSafe(r,s,e',t)
-      requires SemanticSubty(t,Type.Bool(AnyBool))
-      ensures IsSafe(r,s,Or(e,e'),t)
-    {
-      if Evaluate(e,r,s).Ok? && Evaluate(e',r,s).Ok? {
-        assert Evaluate(e,r,s) == base.Ok(Value.Primitive(Primitive.Bool(false)));
-        var v :| Evaluate(e',r,s) == base.Ok(v) && InstanceOfType(v,t);
-        assert InstanceOfType(v,Type.Bool(AnyBool)) by {
-          SemSubtyTransportVal(t,Type.Bool(AnyBool),v);
-        }
-        var b :| v == Value.Primitive(Primitive.Bool(b));
-        assert Evaluator(r,s).interpretShortcircuit(Or(e,e'),e,e',true) == base.Ok(Value.Primitive(Primitive.Bool(b)));
-        assert Evaluate(Or(e,e'),r,s) == base.Ok(Value.Primitive(Primitive.Bool(b)));
-        assert IsSafe(r,s,e',Type.Bool(AnyBool)) by {
-          SemSubtyTransport(r,s,e',t,Type.Bool(AnyBool));
-        }
+  lemma OrRRetSafe(r: Request, s: EntityStore, e: Expr, e': Expr, t: Type)
+    requires IsFalse(r,s,e)
+    requires IsSafe(r,s,e',t)
+    requires SemanticSubty(t,Type.Bool(AnyBool))
+    ensures IsSafe(r,s,Or(e,e'),t)
+  {
+    reveal IsSafe();
+    if Evaluate(e,r,s).Ok? && Evaluate(e',r,s).Ok? {
+      assert Evaluate(e,r,s) == base.Ok(Value.Primitive(Primitive.Bool(false)));
+      var v :| Evaluate(e',r,s) == base.Ok(v) && InstanceOfType(v,t);
+      assert InstanceOfType(v,Type.Bool(AnyBool)) by {
+        SemSubtyTransportVal(t,Type.Bool(AnyBool),v);
+      }
+      var b :| v == Value.Primitive(Primitive.Bool(b));
+      assert Evaluator(r,s).interpretShortcircuit(Or(e,e'),e,e',true) == base.Ok(Value.Primitive(Primitive.Bool(b)));
+      assert Evaluate(Or(e,e'),r,s) == base.Ok(Value.Primitive(Primitive.Bool(b)));
+      assert IsSafe(r,s,e',Type.Bool(AnyBool)) by {
+        SemSubtyTransport(r,s,e',t,Type.Bool(AnyBool));
+      }
+    } else {
+      if Evaluate(e,r,s).Err? {
+        assert Evaluator(r,s).interpretShortcircuit(Or(e,e'),e,e',true) == Evaluate(e,r,s);
+        assert Evaluate(Or(e,e'),r,s) == Evaluate(e,r,s);
       } else {
-        if Evaluate(e,r,s).Err? {
-          assert Evaluator(r,s).interpretShortcircuit(Or(e,e'),e,e',true) == Evaluate(e,r,s);
-          assert Evaluate(Or(e,e'),r,s) == Evaluate(e,r,s);
+        assert Evaluate(e',r,s).Err?;
+        var b :| Evaluate(e,r,s) == base.Ok(Value.Primitive(Primitive.Bool(b)));
+        if b {
+          assert Evaluator(r,s).interpretShortcircuit(Or(e,e'),e,e',true) == base.Ok(Value.Primitive(Primitive.Bool(true)));
+          assert Evaluate(Or(e,e'),r,s) == base.Ok(Value.Primitive(Primitive.Bool(true)));
         } else {
-          assert Evaluate(e',r,s).Err?;
-          var b :| Evaluate(e,r,s) == base.Ok(Value.Primitive(Primitive.Bool(b)));
-          if b {
-            assert Evaluator(r,s).interpretShortcircuit(Or(e,e'),e,e',true) == base.Ok(Value.Primitive(Primitive.Bool(true)));
-            assert Evaluate(Or(e,e'),r,s) == base.Ok(Value.Primitive(Primitive.Bool(true)));
-          } else {
-            assert Evaluator(r,s).interpretShortcircuit(Or(e,e'),e,e',true) == Evaluate(e',r,s);
-            assert Evaluate(Or(e,e'),r,s) == Evaluate(e',r,s);
-          }
+          assert Evaluator(r,s).interpretShortcircuit(Or(e,e'),e,e',true) == Evaluate(e',r,s);
+          assert Evaluate(Or(e,e'),r,s) == Evaluate(e',r,s);
         }
       }
     }
+  }
 
-    lemma OrSafe(r: Request, s: EntityStore, e: Expr, e': Expr)
-      requires IsSafe(r,s,e,Type.Bool(AnyBool))
-      requires IsSafe(r,s,e',Type.Bool(AnyBool))
-      ensures IsSafe(r,s,Or(e,e'),Type.Bool(AnyBool))
-    {
-      if Evaluate(e,r,s).Ok? && Evaluate(e',r,s).Ok? {
-        assert Evaluator(r,s).interpretShortcircuit(Or(e,e'),e,e',true).Ok?;
-        assert Evaluate(Or(e,e'),r,s).Ok?;
+  lemma OrSafe(r: Request, s: EntityStore, e: Expr, e': Expr)
+    requires IsSafe(r,s,e,Type.Bool(AnyBool))
+    requires IsSafe(r,s,e',Type.Bool(AnyBool))
+    ensures IsSafe(r,s,Or(e,e'),Type.Bool(AnyBool))
+  {
+    reveal IsSafe();
+    if Evaluate(e,r,s).Ok? && Evaluate(e',r,s).Ok? {
+      assert Evaluator(r,s).interpretShortcircuit(Or(e,e'),e,e',true).Ok?;
+      assert Evaluate(Or(e,e'),r,s).Ok?;
+    } else {
+      if Evaluate(e,r,s).Err? {
+        assert Evaluator(r,s).interpretShortcircuit(Or(e,e'),e,e',true) == Evaluate(e,r,s);
+        assert Evaluate(Or(e,e'),r,s) == Evaluate(e,r,s);
       } else {
-        if Evaluate(e,r,s).Err? {
-          assert Evaluator(r,s).interpretShortcircuit(Or(e,e'),e,e',true) == Evaluate(e,r,s);
-          assert Evaluate(Or(e,e'),r,s) == Evaluate(e,r,s);
+        assert Evaluate(e',r,s).Err?;
+        var b :| Evaluate(e,r,s) == base.Ok(Value.Primitive(Primitive.Bool(b)));
+        if b {
+          assert Evaluator(r,s).interpretShortcircuit(Or(e,e'),e,e',true) == base.Ok(Value.Primitive(Primitive.Bool(true)));
+          assert Evaluate(Or(e,e'),r,s) == base.Ok(Value.Primitive(Primitive.Bool(true)));
         } else {
-          assert Evaluate(e',r,s).Err?;
-          var b :| Evaluate(e,r,s) == base.Ok(Value.Primitive(Primitive.Bool(b)));
-          if b {
-            assert Evaluator(r,s).interpretShortcircuit(Or(e,e'),e,e',true) == base.Ok(Value.Primitive(Primitive.Bool(true)));
-            assert Evaluate(Or(e,e'),r,s) == base.Ok(Value.Primitive(Primitive.Bool(true)));
-          } else {
-            assert Evaluator(r,s).interpretShortcircuit(Or(e,e'),e,e',true) == Evaluate(e',r,s);
-            assert Evaluate(Or(e,e'),r,s) == Evaluate(e',r,s);
-          }
+          assert Evaluator(r,s).interpretShortcircuit(Or(e,e'),e,e',true) == Evaluate(e',r,s);
+          assert Evaluate(Or(e,e'),r,s) == Evaluate(e',r,s);
         }
       }
     }
+  }
 
-    lemma OrTrueStrong(r: Request, s: EntityStore, e1: Expr, e2: Expr)
-      requires IsTrueStrong(r,s,Or(e1,e2))
-      ensures IsTrueStrong(r,s,e1) || IsTrueStrong(r,s,e2)
-    {
-      assert Evaluator(r,s).interpretShortcircuit(Or(e1,e2),e1,e2,true) == base.Ok(Value.Bool(true));
-    }
+  lemma OrTrueStrong(r: Request, s: EntityStore, e1: Expr, e2: Expr)
+    requires IsTrueStrong(r,s,Or(e1,e2))
+    ensures IsTrueStrong(r,s,e1) || IsTrueStrong(r,s,e2)
+  {
+    reveal IsSafeStrong();
+    reveal IsSafe();
+    assert Evaluator(r,s).interpretShortcircuit(Or(e1,e2),e1,e2,true) == base.Ok(Value.Bool(true));
+  }
 
-    lemma NotTrueSafe(r: Request, s: EntityStore, e: Expr)
-      requires IsTrue(r,s,e)
-      ensures IsFalse(r,s,UnaryApp(Not,e))
-    {}
+  lemma NotTrueSafe(r: Request, s: EntityStore, e: Expr)
+    requires IsTrue(r,s,e)
+    ensures IsFalse(r,s,UnaryApp(Not,e))
+  {
+    reveal IsSafe();
+  }
 
-    lemma NotFalseSafe(r: Request, s: EntityStore, e: Expr)
-      requires IsFalse(r,s,e)
-      ensures IsTrue(r,s,UnaryApp(Not,e))
-    {}
+  lemma NotFalseSafe(r: Request, s: EntityStore, e: Expr)
+    requires IsFalse(r,s,e)
+    ensures IsTrue(r,s,UnaryApp(Not,e))
+  {
+    reveal IsSafe();
+  }
 
-    lemma NotSafe(r: Request, s: EntityStore, e: Expr)
-      requires IsSafe(r,s,e,Type.Bool(AnyBool))
-      ensures IsSafe(r,s,UnaryApp(Not,e),Type.Bool(AnyBool))
-    {}
+  lemma NotSafe(r: Request, s: EntityStore, e: Expr)
+    requires IsSafe(r,s,e,Type.Bool(AnyBool))
+    ensures IsSafe(r,s,UnaryApp(Not,e),Type.Bool(AnyBool))
+  {
+    reveal IsSafe();
+  }
 
-    lemma NegSafe(r: Request, s: EntityStore, e: Expr)
-      requires IsSafe(r,s,e,Type.Int)
-      ensures IsSafe(r,s,UnaryApp(Neg,e),Type.Int)
-    {}
+  lemma NegSafe(r: Request, s: EntityStore, e: Expr)
+    requires IsSafe(r,s,e,Type.Int)
+    ensures IsSafe(r,s,UnaryApp(Neg,e),Type.Int)
+  {
+    reveal IsSafe();
+  }
 
-    lemma MulBySafe(r: Request, s: EntityStore, e: Expr, i: int)
-      requires IsSafe(r,s,e,Type.Int)
-      ensures IsSafe(r,s,UnaryApp(MulBy(i),e),Type.Int)
-    {}
+  lemma MulBySafe(r: Request, s: EntityStore, e: Expr, i: int)
+    requires IsSafe(r,s,e,Type.Int)
+    ensures IsSafe(r,s,UnaryApp(MulBy(i),e),Type.Int)
+  {
+    reveal IsSafe();
+  }
 
-    lemma IteTrueSafe(r: Request, s: EntityStore, e: Expr, e1: Expr, e2: Expr, t: Type)
-      requires IsTrue(r,s,e)
-      requires IsSafe(r,s,e1,t)
-      ensures IsSafe(r,s,If(e,e1,e2),t)
-    {}
+  lemma IteTrueSafe(r: Request, s: EntityStore, e: Expr, e1: Expr, e2: Expr, t: Type)
+    requires IsTrue(r,s,e)
+    requires IsSafe(r,s,e1,t)
+    ensures IsSafe(r,s,If(e,e1,e2),t)
+  {
+    reveal IsSafe();
+  }
 
-    lemma IteFalseSafe(r: Request, s: EntityStore, e: Expr, e1: Expr, e2: Expr, t: Type)
-      requires IsFalse(r,s,e)
-      requires IsSafe(r,s,e2,t)
-      ensures IsSafe(r,s,If(e,e1,e2),t)
-    {}
+  lemma IteFalseSafe(r: Request, s: EntityStore, e: Expr, e1: Expr, e2: Expr, t: Type)
+    requires IsFalse(r,s,e)
+    requires IsSafe(r,s,e2,t)
+    ensures IsSafe(r,s,If(e,e1,e2),t)
+  {
+    reveal IsSafe();
+  }
 
-    lemma IteTrueStrongTrue(r: Request, s: EntityStore, e1: Expr, e2: Expr, e3: Expr)
-      requires IsTrue(r,s,e1)
-      requires IsTrueStrong(r,s,If(e1,e2,e3))
-      ensures IsTrueStrong(r,s,e2)
-    {}
+  lemma IteTrueStrongTrue(r: Request, s: EntityStore, e1: Expr, e2: Expr, e3: Expr)
+    requires IsTrue(r,s,e1)
+    requires IsTrueStrong(r,s,If(e1,e2,e3))
+    ensures IsTrueStrong(r,s,e2)
+  {
+    reveal IsSafeStrong();
+    reveal IsSafe();
+  }
 
-    lemma IteTrueStrongFalse(r: Request, s: EntityStore, e1: Expr, e2: Expr, e3: Expr)
-      requires IsFalse(r,s,e1)
-      requires IsTrueStrong(r,s,If(e1,e2,e3))
-      ensures IsTrueStrong(r,s,e3)
-    {}
+  lemma IteTrueStrongFalse(r: Request, s: EntityStore, e1: Expr, e2: Expr, e3: Expr)
+    requires IsFalse(r,s,e1)
+    requires IsTrueStrong(r,s,If(e1,e2,e3))
+    ensures IsTrueStrong(r,s,e3)
+  {
+    reveal IsSafeStrong();
+    reveal IsSafe();
+  }
 
-    lemma IteError(r: Request, s: EntityStore, e1: Expr, e2: Expr, e3: Expr, t: Type, tnew: Type)
-      requires IsSafe(r,s,e1,t)
-      requires !IsSafeStrong(r,s,e1,t)
-      ensures IsSafe(r,s,If(e1,e2,e3),tnew)
-      ensures !IsSafeStrong(r,s,If(e1,e2,e3),tnew)
-    {}
+  lemma IteError(r: Request, s: EntityStore, e1: Expr, e2: Expr, e3: Expr, t: Type, tnew: Type)
+    requires IsSafe(r,s,e1,t)
+    requires !IsSafeStrong(r,s,e1,t)
+    ensures IsSafe(r,s,If(e1,e2,e3),tnew)
+    ensures !IsSafeStrong(r,s,If(e1,e2,e3),tnew)
+  {
+    reveal IsSafeStrong();
+    reveal IsSafe();
+  }
 
-    lemma ContainsSetSafe(r: Request, s: EntityStore, e: Expr, e': Expr, t1: Type, t2: Type)
-      requires IsSafe(r,s,e,Type.Set(t1))
-      requires IsSafe(r,s,e',t2)
-      ensures IsSafe(r,s,BinaryApp(Contains,e,e'),Type.Bool(AnyBool))
-    {}
+  lemma ContainsSetSafe(r: Request, s: EntityStore, e: Expr, e': Expr, t1: Type, t2: Type)
+    requires IsSafe(r,s,e,Type.Set(t1))
+    requires IsSafe(r,s,e',t2)
+    ensures IsSafe(r,s,BinaryApp(Contains,e,e'),Type.Bool(AnyBool))
+  {
+    reveal IsSafe();
+  }
 
-    lemma LikeSafe(r: Request, s: EntityStore, e: Expr, p: Pattern)
-      requires IsSafe(r,s,e,Type.String)
-      ensures IsSafe(r,s,UnaryApp(Like(p),e),Type.Bool(AnyBool))
-    {}
+  lemma LikeSafe(r: Request, s: EntityStore, e: Expr, p: Pattern)
+    requires IsSafe(r,s,e,Type.String)
+    ensures IsSafe(r,s,UnaryApp(Like(p),e),Type.Bool(AnyBool))
+  {
+    reveal IsSafe();
+  }
 
-    lemma SetConstrSafe(r: Request, s: EntityStore, es: seq<Expr>, t: Type)
-      requires forall i :: 0 <= i < |es| ==> IsSafe(r,s,es[i],t)
-      ensures IsSafe(r,s,Expr.Set(es),Type.Set(t))
-    {
-      InterpretSetLemma(es,r,s);
-      if(forall i :: 0 <= i < |es| ==> exists v :: Evaluate(es[i],r,s) == base.Ok(v) && InstanceOfType(v,t)){
-        assert forall e :: e in es ==> Evaluate(e,r,s).Ok?;
-        assert Evaluate(Expr.Set(es),r,s).Ok?;
-        var vs :| Evaluator(r,s).interpretSet(es) == base.Ok(vs);
-        assert InstanceOfType(Value.Set(vs),Type.Set(t)) by {
-          forall v | v in vs ensures InstanceOfType(v,t) {}
-        }
+  lemma SetConstrSafe(r: Request, s: EntityStore, es: seq<Expr>, t: Type)
+    requires forall i :: 0 <= i < |es| ==> IsSafe(r,s,es[i],t)
+    ensures IsSafe(r,s,Expr.Set(es),Type.Set(t))
+  {
+    reveal IsSafe();
+    InterpretSetLemma(es,r,s);
+    if(forall i :: 0 <= i < |es| ==> exists v :: Evaluate(es[i],r,s) == base.Ok(v) && InstanceOfType(v,t)){
+      assert forall e :: e in es ==> Evaluate(e,r,s).Ok?;
+      assert Evaluate(Expr.Set(es),r,s).Ok?;
+      var vs :| Evaluator(r,s).interpretSet(es) == base.Ok(vs);
+      assert InstanceOfType(Value.Set(vs),Type.Set(t)) by {
+        forall v | v in vs ensures InstanceOfType(v,t) {}
       }
     }
+  }
 
-    lemma ContainsAnyAllSafe(r: Request, s: EntityStore, op: BinaryOp, e1: Expr, e2: Expr, t1: Type, t2: Type)
-      requires op == ContainsAll || op == ContainsAny
-      requires IsSafe(r,s,e1,Type.Set(t1))
-      requires IsSafe(r,s,e2,Type.Set(t2))
-      ensures IsSafe(r,s,BinaryApp(op,e1,e2), Type.Bool(AnyBool))
-    {}
+  lemma ContainsAnyAllSafe(r: Request, s: EntityStore, op: BinaryOp, e1: Expr, e2: Expr, t1: Type, t2: Type)
+    requires op == ContainsAll || op == ContainsAny
+    requires IsSafe(r,s,e1,Type.Set(t1))
+    requires IsSafe(r,s,e2,Type.Set(t2))
+    ensures IsSafe(r,s,BinaryApp(op,e1,e2), Type.Bool(AnyBool))
+  {
+    reveal IsSafe();
+  }
 
-    lemma IneqSafe(r: Request, s: EntityStore, op: BinaryOp, e1: Expr, e2: Expr)
-      requires op == Less || op == BinaryOp.LessEq
-      requires IsSafe(r,s,e1,Type.Int)
-      requires IsSafe(r,s,e2,Type.Int)
-      ensures IsSafe(r,s,BinaryApp(op,e1,e2),Type.Bool(AnyBool))
-    {}
+  lemma IneqSafe(r: Request, s: EntityStore, op: BinaryOp, e1: Expr, e2: Expr)
+    requires op == Less || op == BinaryOp.LessEq
+    requires IsSafe(r,s,e1,Type.Int)
+    requires IsSafe(r,s,e2,Type.Int)
+    ensures IsSafe(r,s,BinaryApp(op,e1,e2),Type.Bool(AnyBool))
+  {
+    reveal IsSafe();
+  }
 
-    lemma ArithSafe(r: Request, s: EntityStore, op: BinaryOp, e1: Expr, e2: Expr)
-      requires op == Add || op == Sub
-      requires IsSafe(r,s,e1,Type.Int)
-      requires IsSafe(r,s,e2,Type.Int)
-      ensures IsSafe(r,s,BinaryApp(op,e1,e2),Type.Int)
-    {}
+  lemma ArithSafe(r: Request, s: EntityStore, op: BinaryOp, e1: Expr, e2: Expr)
+    requires op == Add || op == Sub
+    requires IsSafe(r,s,e1,Type.Int)
+    requires IsSafe(r,s,e2,Type.Int)
+    ensures IsSafe(r,s,BinaryApp(op,e1,e2),Type.Int)
+  {
+    reveal IsSafe();
+  }
 
-    // We prove that every extension function is safe with respect to the
-    // ExtFunType assigned to it by the validator. In particular, we show that
-    // the argument types of the ExtFunType match the argument type checks
-    // actually performed by the function at runtime, the return value has the
-    // correct type on success, and the function doesn't raise any error other
-    // than ExtensionError.
-    //
-    // Writing one lemma per extension function would be a lot of boilerplate.
-    // Instead, we put them in groups that have the same ExtFunType.
+  // We prove that every extension function is safe with respect to the
+  // ExtFunType assigned to it by the validator. In particular, we show that
+  // the argument types of the ExtFunType match the argument type checks
+  // actually performed by the function at runtime, the return value has the
+  // correct type on success, and the function doesn't raise any error other
+  // than ExtensionError.
+  //
+  // Writing one lemma per extension function would be a lot of boilerplate.
+  // Instead, we put them in groups that have the same ExtFunType.
 
-    ghost predicate ExtensionFunSafeRequires(name: base.Name, args: seq<Value>)
-      requires name in extFunTypes
-    {
-      var eft := extFunTypes[name];
-      |args| == |eft.args| &&
-      forall i | 0 <= i < |args| :: InstanceOfType(args[i], eft.args[i])
-    }
+  ghost predicate ExtensionFunSafeRequires(name: base.Name, args: seq<Value>)
+    requires name in extFunTypes
+  {
+    var eft := extFunTypes[name];
+    |args| == |eft.args| &&
+    forall i | 0 <= i < |args| :: InstanceOfType(args[i], eft.args[i])
+  }
 
-    ghost predicate ExtensionFunSafeEnsures(name: base.Name, args: seq<Value>)
-      requires name in extFunTypes
-    {
-      var eft := extFunTypes[name];
-      var res := extFuns[name].fun(args);
-      res == base.Err(base.ExtensionError) || (res.Ok? && InstanceOfType(res.value, eft.ret))
-    }
+  ghost predicate ExtensionFunSafeEnsures(name: base.Name, args: seq<Value>)
+    requires name in extFunTypes
+  {
+    var eft := extFunTypes[name];
+    var res := extFuns[name].fun(args);
+    res == base.Err(base.ExtensionError) || (res.Ok? && InstanceOfType(res.value, eft.ret))
+  }
 
-    ghost predicate IsDecimalConstructorName(name: base.Name) {
-      name == base.Name.fromStr("decimal")
-    }
+  ghost predicate IsDecimalConstructorName(name: base.Name) {
+    name == base.Name.fromStr("decimal")
+  }
 
-    lemma DecimalConstructorSafe(name: base.Name, args: seq<Value>)
-      requires IsDecimalConstructorName(name)
-      requires ExtensionFunSafeRequires(name, args)
-      ensures ExtensionFunSafeEnsures(name, args)
-    {}
+  lemma DecimalConstructorSafe(name: base.Name, args: seq<Value>)
+    requires IsDecimalConstructorName(name)
+    requires ExtensionFunSafeRequires(name, args)
+    ensures ExtensionFunSafeEnsures(name, args)
+  {}
 
-    ghost predicate IsDecimalComparisonName(name: base.Name) {
-      name == base.Name.fromStr("lessThan") ||
-      name == base.Name.fromStr("lessThanOrEqual") ||
-      name == base.Name.fromStr("greaterThan") ||
-      name == base.Name.fromStr("greaterThanOrEqual")
-    }
+  ghost predicate IsDecimalComparisonName(name: base.Name) {
+    name == base.Name.fromStr("lessThan") ||
+    name == base.Name.fromStr("lessThanOrEqual") ||
+    name == base.Name.fromStr("greaterThan") ||
+    name == base.Name.fromStr("greaterThanOrEqual")
+  }
 
-    lemma DecimalComparisonSafe(name: base.Name, args: seq<Value>)
-      requires IsDecimalComparisonName(name)
-      requires ExtensionFunSafeRequires(name, args)
-      ensures ExtensionFunSafeEnsures(name, args)
-    {}
+  lemma DecimalComparisonSafe(name: base.Name, args: seq<Value>)
+    requires IsDecimalComparisonName(name)
+    requires ExtensionFunSafeRequires(name, args)
+    ensures ExtensionFunSafeEnsures(name, args)
+  {}
 
-    ghost predicate IsIpConstructorName(name: base.Name) {
-      name == base.Name.fromStr("ip")
-    }
+  ghost predicate IsIpConstructorName(name: base.Name) {
+    name == base.Name.fromStr("ip")
+  }
 
-    lemma IpConstructorSafe(name: base.Name, args: seq<Value>)
-      requires IsIpConstructorName(name)
-      requires ExtensionFunSafeRequires(name, args)
-      ensures ExtensionFunSafeEnsures(name, args)
-    {}
+  lemma IpConstructorSafe(name: base.Name, args: seq<Value>)
+    requires IsIpConstructorName(name)
+    requires ExtensionFunSafeRequires(name, args)
+    ensures ExtensionFunSafeEnsures(name, args)
+  {}
 
-    ghost predicate IsIpUnaryName(name: base.Name) {
-      name == base.Name.fromStr("isIpv4") ||
-      name == base.Name.fromStr("isIpv6") ||
-      name == base.Name.fromStr("isLoopback") ||
-      name == base.Name.fromStr("isMulticast")
-    }
+  ghost predicate IsIpUnaryName(name: base.Name) {
+    name == base.Name.fromStr("isIpv4") ||
+    name == base.Name.fromStr("isIpv6") ||
+    name == base.Name.fromStr("isLoopback") ||
+    name == base.Name.fromStr("isMulticast")
+  }
 
-    lemma IpUnarySafe(name: base.Name, args: seq<Value>)
-      requires IsIpUnaryName(name)
-      requires ExtensionFunSafeRequires(name, args)
-      ensures ExtensionFunSafeEnsures(name, args)
-    {
-      assert |args| == 1 && args[0].Extension? && args[0].ex.IPAddr?;
-    }
+  lemma IpUnarySafe(name: base.Name, args: seq<Value>)
+    requires IsIpUnaryName(name)
+    requires ExtensionFunSafeRequires(name, args)
+    ensures ExtensionFunSafeEnsures(name, args)
+  {
+    assert |args| == 1 && args[0].Extension? && args[0].ex.IPAddr?;
+  }
 
-    ghost predicate IsIpBinaryName(name: base.Name) {
-      name == base.Name.fromStr("isInRange")
-    }
+  ghost predicate IsIpBinaryName(name: base.Name) {
+    name == base.Name.fromStr("isInRange")
+  }
 
-    lemma IpBinarySafe(name: base.Name, args: seq<Value>)
-      requires IsIpBinaryName(name)
-      requires ExtensionFunSafeRequires(name, args)
-      ensures ExtensionFunSafeEnsures(name, args)
-    {}
+  lemma IpBinarySafe(name: base.Name, args: seq<Value>)
+    requires IsIpBinaryName(name)
+    requires ExtensionFunSafeRequires(name, args)
+    ensures ExtensionFunSafeEnsures(name, args)
+  {}
 
-    lemma InterpretListEnsures(eval: Evaluator, es: seq<Expr>)
-      ensures eval.interpretList(es).Ok? ==> (|eval.interpretList(es).value| == |es| &&
-                                              forall i | 0 <= i < |es| :: eval.interpret(es[i]) == base.Ok(eval.interpretList(es).value[i]))
-      ensures (forall e :: e in es ==> eval.interpret(e).Ok?) ==> eval.interpretList(es).Ok?
-      ensures (exists i :: 0 <= i < |es| && eval.interpret(es[i]).Err?) ==> eval.interpretList(es).Err?
-      ensures eval.interpretList(es).Err? <==> exists i :: 0 <= i < |es| && eval.interpret(es[i]).Err? && (forall j :: 0 <= j < i ==> eval.interpret(es[j]).Ok?)
-      ensures eval.interpretList(es).Err? ==> exists i :: 0 <= i < |es| && eval.interpret(es[i]).Err? && eval.interpret(es[i]).error == eval.interpretList(es).error && (forall j :: 0 <= j < i ==> eval.interpret(es[j]).Ok?)
-    {}
+  lemma InterpretListEnsures(eval: Evaluator, es: seq<Expr>)
+    ensures eval.interpretList(es).Ok? ==> (|eval.interpretList(es).value| == |es| &&
+                                            forall i | 0 <= i < |es| :: eval.interpret(es[i]) == base.Ok(eval.interpretList(es).value[i]))
+    ensures (forall e :: e in es ==> eval.interpret(e).Ok?) ==> eval.interpretList(es).Ok?
+    ensures (exists i :: 0 <= i < |es| && eval.interpret(es[i]).Err?) ==> eval.interpretList(es).Err?
+    ensures eval.interpretList(es).Err? <==> exists i :: 0 <= i < |es| && eval.interpret(es[i]).Err? && (forall j :: 0 <= j < i ==> eval.interpret(es[j]).Ok?)
+    ensures eval.interpretList(es).Err? ==> exists i :: 0 <= i < |es| && eval.interpret(es[i]).Err? && eval.interpret(es[i]).error == eval.interpretList(es).error && (forall j :: 0 <= j < i ==> eval.interpret(es[j]).Ok?)
+  {}
 
-    lemma CallSafe(r: Request, s: EntityStore, name: base.Name, args: seq<Expr>)
-      requires name in extFunTypes
-      requires |args| == |extFunTypes[name].args|
-      requires forall i | 0 <= i < |args| :: IsSafe(r,s,args[i],extFunTypes[name].args[i])
-      ensures IsSafe(r,s,Call(name,args),extFunTypes[name].ret)
-    {
-      var eft := extFunTypes[name];
-      if (forall i | 0 <= i < |args| :: Evaluate(args[i],r,s).Ok?) {
-        assert forall e <- args :: Evaluate(e,r,s).Ok?;
+  lemma CallSafe(r: Request, s: EntityStore, name: base.Name, args: seq<Expr>)
+    requires name in extFunTypes
+    requires |args| == |extFunTypes[name].args|
+    requires forall i | 0 <= i < |args| :: IsSafe(r,s,args[i],extFunTypes[name].args[i])
+    ensures IsSafe(r,s,Call(name,args),extFunTypes[name].ret)
+  {
+    reveal IsSafe();
+    var eft := extFunTypes[name];
+    if (forall i | 0 <= i < |args| :: Evaluate(args[i],r,s).Ok?) {
+      assert forall e <- args :: Evaluate(e,r,s).Ok?;
 
-        InterpretListEnsures(Evaluator(r, s), args);
-        var argVals := Evaluator(r, s).interpretList(args).value;
+      InterpretListEnsures(Evaluator(r, s), args);
+      var argVals := Evaluator(r, s).interpretList(args).value;
 
-        var res := Evaluator(r, s).applyExtFun(name, argVals);
-        assert Evaluate(Call(name,args),r,s) == res;
-        assert forall i | 0 <= i < |args| :: InstanceOfType(argVals[i], eft.args[i]);
-        var isSafe := (res == base.Err(base.ExtensionError) || (res.Ok? && InstanceOfType(res.value, eft.ret)));
-        if IsDecimalConstructorName(name) {
-          DecimalConstructorSafe(name, argVals);
-          assert isSafe;
-        } else if IsDecimalComparisonName(name) {
-          DecimalComparisonSafe(name, argVals);
-          assert isSafe;
-        } else if IsIpConstructorName(name) {
-          IpConstructorSafe(name, argVals);
-          assert isSafe;
-        } else if IsIpUnaryName(name) {
-          IpUnarySafe(name, argVals);
-          assert isSafe;
-        } else if IsIpBinaryName(name) {
-          IpBinarySafe(name, argVals);
-          assert isSafe;
-        }
-      } else {
-        InterpretListEnsures(Evaluator(r, s), args);
+      var res := Evaluator(r, s).applyExtFun(name, argVals);
+      assert Evaluate(Call(name,args),r,s) == res;
+      assert forall i | 0 <= i < |args| :: InstanceOfType(argVals[i], eft.args[i]);
+      var isSafe := (res == base.Err(base.ExtensionError) || (res.Ok? && InstanceOfType(res.value, eft.ret)));
+      if IsDecimalConstructorName(name) {
+        DecimalConstructorSafe(name, argVals);
+        assert isSafe;
+      } else if IsDecimalComparisonName(name) {
+        DecimalComparisonSafe(name, argVals);
+        assert isSafe;
+      } else if IsIpConstructorName(name) {
+        IpConstructorSafe(name, argVals);
+        assert isSafe;
+      } else if IsIpUnaryName(name) {
+        IpUnarySafe(name, argVals);
+        assert isSafe;
+      } else if IsIpBinaryName(name) {
+        IpBinarySafe(name, argVals);
+        assert isSafe;
       }
+    } else {
+      InterpretListEnsures(Evaluator(r, s), args);
     }
+  }
 
-    lemma RecordSafe(r: Request, s: EntityStore, es: seq<(Attr,Expr)>, rt: RecordType)
-      // every entry has some type
-      requires forall ae :: ae in es ==> exists t :: IsSafe(r,s,ae.1,t)
-      // and the last instance of every required key is safe at the correct type.
-      requires forall k :: k in rt ==> KeyExists(k,es) && IsSafe(r,s,LastOfKey(k,es),rt[k].ty)
-      ensures IsSafe(r,s,Expr.Record(es),Type.Record(rt))
-    {
-      if Evaluator(r,s).interpretRecord(es).Ok? {
-        InterpretRecordLemmaOk(es,r,s);
-      } else {
-        InterpretRecordLemmaErr(es,r,s);
-      }
+  ghost predicate ExistsSafeType(r: Request, s: EntityStore, e: Expr) {
+    exists t :: IsSafe(r,s,e,t)
+  }
+
+  lemma RecordSafe(r: Request, s: EntityStore, es: seq<(Attr,Expr)>, rt: RecordType)
+    // every entry has some type
+    requires forall ae | ae in es :: ExistsSafeType(r,s,ae.1)
+    // and the last instance of every required key is safe at the correct type.
+    requires forall k | k in rt :: KeyExists(k,es) && IsSafe(r,s,LastOfKey(k,es),rt[k].ty)
+    ensures IsSafe(r,s,Expr.Record(es),Type.Record(rt))
+  {
+    reveal IsSafe();
+    if Evaluator(r,s).interpretRecord(es).Ok? {
+      InterpretRecordLemmaOk(es,r,s);
+    } else {
+      InterpretRecordLemmaErr(es,r,s);
     }
+  }
 
-    lemma ObjectProjSafeRequired(r: Request, s: EntityStore, e: Expr, t: Type, l: Attr, t': AttrType)
-      requires IsSafe(r,s,e,t)
-      requires t'.isRequired
-      requires SemanticSubty(t,Type.Record(map[l := t']))
-      ensures IsSafe(r,s,GetAttr(e,l),t'.ty)
-    {}
+  lemma ObjectProjSafeRequired(r: Request, s: EntityStore, e: Expr, t: Type, l: Attr, t': AttrType)
+    requires IsSafe(r,s,e,t)
+    requires t'.isRequired
+    requires SemanticSubty(t,Type.Record(map[l := t']))
+    ensures IsSafe(r,s,GetAttr(e,l),t'.ty)
+  {
+    reveal IsSafe();
+  }
 
-    lemma ObjectProjSafeGetAttrSafe(r: Request, s: EntityStore, e: Expr, t: Type, l: Attr, t': AttrType)
-      requires IsSafe(r,s,e,t)
-      requires SemanticSubty(t,Type.Record(map[l := t']))
-      requires GetAttrSafe(r,s,e,l)
-      ensures IsSafe(r,s,GetAttr(e,l),t'.ty)
-    {}
+  lemma ObjectProjSafeGetAttrSafe(r: Request, s: EntityStore, e: Expr, t: Type, l: Attr, t': AttrType)
+    requires IsSafe(r,s,e,t)
+    requires SemanticSubty(t,Type.Record(map[l := t']))
+    requires GetAttrSafe(r,s,e,l)
+    ensures IsSafe(r,s,GetAttr(e,l),t'.ty)
+  {
+    reveal IsSafe();
+  }
 
-    lemma EntityProjSafe(r: Request, s: EntityStore, e: Expr, l: Attr, lub: EntityLUB, t': Type, isRequired: bool)
-      requires IsSafe(r,s,e,Type.Entity(lub))
-      requires EntityProjStoreCondition(s, l, lub, t', isRequired)
-      requires isRequired || GetAttrSafe(r,s,e,l)
-      ensures IsSafe(r,s,GetAttr(e,l),t')
-    {}
+  lemma EntityProjSafe(r: Request, s: EntityStore, e: Expr, l: Attr, lub: EntityLUB, t': Type, isRequired: bool)
+    requires IsSafe(r,s,e,Type.Entity(lub))
+    requires EntityProjStoreCondition(s, l, lub, t', isRequired)
+    requires isRequired || GetAttrSafe(r,s,e,l)
+    ensures IsSafe(r,s,GetAttr(e,l),t')
+  {
+    reveal IsSafe();
+  }
 
-    lemma RecordHasRequiredTrueSafe(r: Request, s: EntityStore, e: Expr, l: Attr, t: AttrType)
-      requires IsSafe(r,s,e,Type.Record(map[l := t]))
-      requires t.isRequired
-      ensures IsTrue(r,s,HasAttr(e,l))
-    {}
+  lemma RecordHasRequiredTrueSafe(r: Request, s: EntityStore, e: Expr, l: Attr, t: AttrType)
+    requires IsSafe(r,s,e,Type.Record(map[l := t]))
+    requires t.isRequired
+    ensures IsTrue(r,s,HasAttr(e,l))
+  {
+    reveal IsSafe();
+  }
 
-    lemma RecordHasOpenRecSafe(r: Request, s: EntityStore, e: Expr, l: Attr)
-      requires IsSafe(r,s,e,Type.Record(map[]))
-      ensures IsSafe(r,s,HasAttr(e,l),Type.Bool(AnyBool))
-    {}
+  lemma RecordHasOpenRecSafe(r: Request, s: EntityStore, e: Expr, l: Attr)
+    requires IsSafe(r,s,e,Type.Record(map[]))
+    ensures IsSafe(r,s,HasAttr(e,l),Type.Bool(AnyBool))
+  {
+    reveal IsSafe();
+  }
 
-    lemma EntityHasImpossibleFalseSafe(r: Request, s: EntityStore, e: Expr, l: Attr, lub: EntityLUB)
-      requires IsSafe(r,s,e,Type.Entity(lub))
-      requires forall ev: EntityUID | ExistingEntityInLub(s, ev, lub) ::
-                 l !in s.entities[ev].attrs
-      ensures IsFalse(r,s,HasAttr(e,l))
-    {}
+  lemma EntityHasImpossibleFalseSafe(r: Request, s: EntityStore, e: Expr, l: Attr, lub: EntityLUB)
+    requires IsSafe(r,s,e,Type.Entity(lub))
+    requires forall ev: EntityUID | ExistingEntityInLub(s, ev, lub) ::
+                l !in s.entities[ev].attrs
+    ensures IsFalse(r,s,HasAttr(e,l))
+  {
+    reveal IsSafe();
+  }
 
-    lemma EntityHasOpenSafe(r: Request, s: EntityStore, e: Expr, l: Attr)
-      requires IsSafe(r,s,e,Type.Entity(AnyEntity))
-      ensures IsSafe(r,s,HasAttr(e,l),Type.Bool(AnyBool))
-    {}
+  lemma EntityHasOpenSafe(r: Request, s: EntityStore, e: Expr, l: Attr)
+    requires IsSafe(r,s,e,Type.Entity(AnyEntity))
+    ensures IsSafe(r,s,HasAttr(e,l),Type.Bool(AnyBool))
+  {
+    reveal IsSafe();
+  }
 
-    lemma InSingleSafe(r: Request, s: EntityStore, e1: Expr, e2: Expr)
-      requires IsSafe(r,s,e1,Type.Entity(AnyEntity))
-      requires IsSafe(r,s,e2,Type.Entity(AnyEntity))
-      ensures IsSafe(r,s,BinaryApp(BinaryOp.In,e1,e2),Type.Bool(AnyBool))
-    {}
+  lemma InSingleSafe(r: Request, s: EntityStore, e1: Expr, e2: Expr)
+    requires IsSafe(r,s,e1,Type.Entity(AnyEntity))
+    requires IsSafe(r,s,e2,Type.Entity(AnyEntity))
+    ensures IsSafe(r,s,BinaryApp(BinaryOp.In,e1,e2),Type.Bool(AnyBool))
+  {
+    reveal IsSafe();
+  }
 
-    lemma EntityInEntityMatchesEngine(r: Request, s: EntityStore, u1: EntityUID, u2: EntityUID)
-      ensures EntityInEntity(s,u1,u2) == Evaluator(r,s).entityInEntity(u1,u2)
-    {}
+  lemma EntityInEntityMatchesEngine(r: Request, s: EntityStore, u1: EntityUID, u2: EntityUID)
+    ensures EntityInEntity(s,u1,u2) == Evaluator(r,s).entityInEntity(u1,u2)
+  {}
 
-    lemma InSingleFalseLiterals(r: Request, s: EntityStore, u1: EntityUID, u2: EntityUID)
-      requires !EntityInEntity(s,u1,u2)
-      ensures IsFalse(r,s,BinaryApp(BinaryOp.In,PrimitiveLit(Primitive.EntityUID(u1)),PrimitiveLit(Primitive.EntityUID(u2))))
-    {
-      var evaluator := Evaluator(r,s);
-      calc == {
-        evaluator.interpret(BinaryApp(BinaryOp.In,PrimitiveLit(Primitive.EntityUID(u1)),PrimitiveLit(Primitive.EntityUID(u2))));
-        evaluator.applyBinaryOp(BinaryOp.In,Value.EntityUID(u1),Value.EntityUID(u2));
-        base.Ok(Value.Bool(evaluator.entityInEntity(u1, u2)));
-      }
+  lemma InSingleFalseLiterals(r: Request, s: EntityStore, u1: EntityUID, u2: EntityUID)
+    requires !EntityInEntity(s,u1,u2)
+    ensures IsFalse(r,s,BinaryApp(BinaryOp.In,PrimitiveLit(Primitive.EntityUID(u1)),PrimitiveLit(Primitive.EntityUID(u2))))
+  {
+    reveal IsSafe();
+    var evaluator := Evaluator(r,s);
+    calc == {
+      evaluator.interpret(BinaryApp(BinaryOp.In,PrimitiveLit(Primitive.EntityUID(u1)),PrimitiveLit(Primitive.EntityUID(u2))));
+      evaluator.applyBinaryOp(BinaryOp.In,Value.EntityUID(u1),Value.EntityUID(u2));
+      base.Ok(Value.Bool(evaluator.entityInEntity(u1, u2)));
     }
+  }
 
-    lemma InSingleFalseEntityTypeAndLiteral(r: Request, s: EntityStore, e1: Expr, et1: EntityType, u2: EntityUID)
-      requires IsSafe(r,s,e1,Type.Entity(EntityLUB({et1})))
-      requires forall u1: EntityUID | u1.ty == et1 :: !EntityInEntity(s,u1,u2)
-      ensures IsFalse(r,s,BinaryApp(BinaryOp.In,e1,PrimitiveLit(Primitive.EntityUID(u2))))
-    {
-      var evaluator := Evaluator(r,s);
-      var r1 := evaluator.interpret(e1);
-      if r1.Ok? {
-        var u1 :- assert Value.asEntity(r1.value);
-        assert u1.ty == et1;
-        assert !EntityInEntity(s,u1,u2);
-        assert evaluator.interpret(BinaryApp(BinaryOp.In,e1,PrimitiveLit(Primitive.EntityUID(u2)))) == base.Ok(Value.FALSE);
-      }
+  lemma InSingleFalseEntityTypeAndLiteral(r: Request, s: EntityStore, e1: Expr, et1: EntityType, u2: EntityUID)
+    requires IsSafe(r,s,e1,Type.Entity(EntityLUB({et1})))
+    requires forall u1: EntityUID | u1.ty == et1 :: !EntityInEntity(s,u1,u2)
+    ensures IsFalse(r,s,BinaryApp(BinaryOp.In,e1,PrimitiveLit(Primitive.EntityUID(u2))))
+  {
+    reveal IsSafe();
+    var evaluator := Evaluator(r,s);
+    var r1 := evaluator.interpret(e1);
+    if r1.Ok? {
+      var u1 :- assert Value.asEntity(r1.value);
+      assert u1.ty == et1;
+      assert !EntityInEntity(s,u1,u2);
+      assert evaluator.interpret(BinaryApp(BinaryOp.In,e1,PrimitiveLit(Primitive.EntityUID(u2)))) == base.Ok(Value.FALSE);
     }
+  }
 
-    lemma InSingleFalseTypes(r: Request, s: EntityStore, e1: Expr, e2: Expr, t1: Type, t2: Type)
-      requires subty(t1,Type.Entity(AnyEntity))
-      requires subty(t2,Type.Entity(AnyEntity))
-      requires IsSafe(r,s,e1,t1)
-      requires IsSafe(r,s,e2,t2)
-      requires forall u1, u2: EntityUID |
-                 InstanceOfType(Value.EntityUID(u1), t1) && InstanceOfType(Value.EntityUID(u2), t2) ::
-                 !EntityInEntity(s,u1,u2)
-      ensures IsFalse(r,s,BinaryApp(BinaryOp.In,e1,e2))
-    {
-      var evaluator := Evaluator(r,s);
-      if evaluator.interpret(BinaryApp(BinaryOp.In,e1,e2)).Ok? {
-        var u1 := Value.asEntity(evaluator.interpret(e1).value).value;
-        var u2 := Value.asEntity(evaluator.interpret(e2).value).value;
-        assert !EntityInEntity(s,u1,u2);
-      }
+  lemma InSingleFalseTypes(r: Request, s: EntityStore, e1: Expr, e2: Expr, t1: Type, t2: Type)
+    requires subty(t1,Type.Entity(AnyEntity))
+    requires subty(t2,Type.Entity(AnyEntity))
+    requires IsSafe(r,s,e1,t1)
+    requires IsSafe(r,s,e2,t2)
+    requires forall u1, u2: EntityUID |
+      InstanceOfType(Value.EntityUID(u1), t1) && InstanceOfType(Value.EntityUID(u2), t2) ::
+      !EntityInEntity(s,u1,u2)
+    ensures IsFalse(r,s,BinaryApp(BinaryOp.In,e1,e2))
+  {
+    var evaluator := Evaluator(r,s);
+    var r1 := evaluator.interpret(e1);
+    var r2 := evaluator.interpret(e2);
+    var res := evaluator.interpret(BinaryApp(BinaryOp.In,e1,e2));
+
+    reveal IsSafe();
+    if r1.Err? {
+      assert res == r1;
+    } else if r2.Err? {
+      assert res == r2;
+    } else {
+      assert r1.value.Primitive? && r1.value.primitive.EntityUID?;
+      assert r2.value.Primitive? && r2.value.primitive.EntityUID?;
+      var u1 := r1.value.primitive.uid;
+      var u2 := r2.value.primitive.uid;
+      assert !EntityInEntity(s,u1,u2);
+      assert res.value == Value.FALSE;
     }
+  }
 
-    lemma InSetSafe(r: Request, s: EntityStore, e1: Expr, e2: Expr)
-      requires IsSafe(r,s,e1,Type.Entity(AnyEntity))
-      requires IsSafe(r,s,e2,Type.Set(Type.Entity(AnyEntity)))
-      ensures IsSafe(r,s,BinaryApp(BinaryOp.In,e1,e2),Type.Bool(AnyBool))
-    {}
+  lemma InSetSafe(r: Request, s: EntityStore, e1: Expr, e2: Expr)
+    requires IsSafe(r,s,e1,Type.Entity(AnyEntity))
+    requires IsSafe(r,s,e2,Type.Set(Type.Entity(AnyEntity)))
+    ensures IsSafe(r,s,BinaryApp(BinaryOp.In,e1,e2),Type.Bool(AnyBool))
+  {
+    reveal IsSafe();
+  }
 
-    lemma InSetFalseIfAllFalse(r: Request, s: EntityStore, e1: Expr, e2s: seq<Expr>)
-      requires IsSafe(r,s,e1,Type.Entity(AnyEntity))
-      requires forall i | 0 <= i < |e2s| ::
-                 IsSafe(r,s,e2s[i],Type.Entity(AnyEntity)) &&
-                 IsFalse(r,s,BinaryApp(BinaryOp.In,e1,e2s[i]))
-      ensures IsFalse(r,s,BinaryApp(BinaryOp.In,e1,Expr.Set(e2s)))
-    {
-      InterpretSetLemma(e2s,r,s);
-      var evaluator := Evaluator(r,s);
-      var res := evaluator.interpret(BinaryApp(BinaryOp.In,e1,Expr.Set(e2s)));
-      var r1 := evaluator.interpret(e1);
-      var r2 := evaluator.interpret(Expr.Set(e2s));
-    }
+  lemma InSetFalseIfAllFalse(r: Request, s: EntityStore, e1: Expr, e2s: seq<Expr>)
+    requires IsSafe(r,s,e1,Type.Entity(AnyEntity))
+    requires forall i | 0 <= i < |e2s| ::
+                IsSafe(r,s,e2s[i],Type.Entity(AnyEntity)) &&
+                IsFalse(r,s,BinaryApp(BinaryOp.In,e1,e2s[i]))
+    ensures IsFalse(r,s,BinaryApp(BinaryOp.In,e1,Expr.Set(e2s)))
+  {
+    reveal IsSafe();
+    InterpretSetLemma(e2s,r,s);
+    var evaluator := Evaluator(r,s);
+    var res := evaluator.interpret(BinaryApp(BinaryOp.In,e1,Expr.Set(e2s)));
+    var r1 := evaluator.interpret(e1);
+    var r2 := evaluator.interpret(Expr.Set(e2s));
+  }
 
-    lemma InSetFalseTypes(r: Request, s: EntityStore, e1: Expr, e2: Expr, t1: Type, t2: Type)
-      requires subty(t1,Type.Entity(AnyEntity))
-      requires subty(t2,Type.Entity(AnyEntity))
-      requires IsSafe(r,s,e1,t1)
-      requires IsSafe(r,s,e2,Type.Set(t2))
-      requires forall u1, u2: EntityUID |
-                 InstanceOfType(Value.EntityUID(u1), t1) && InstanceOfType(Value.EntityUID(u2), t2) ::
-                 !EntityInEntity(s,u1,u2)
-      ensures IsFalse(r,s,BinaryApp(BinaryOp.In,e1,e2))
-    {
-      var evaluator := Evaluator(r,s);
-      var r1 := evaluator.interpret(e1);
-      var r2 := evaluator.interpret(e2);
-      if r1.Ok? && r2.Ok? {
-        var u1 := Value.asEntity(r1.value).value;
-        var s2 := Value.asSet(r2.value).value;
-        assert forall us2 <- s2 :: InstanceOfType(us2,t2);
-        var us2 :- assert evaluator.checkEntitySet(s2);
-        assert forall u2 <- us2 :: !EntityInEntity(s,u1,u2);
-      }
+  lemma InSetFalseTypes(r: Request, s: EntityStore, e1: Expr, e2: Expr, t1: Type, t2: Type)
+    requires subty(t1,Type.Entity(AnyEntity))
+    requires subty(t2,Type.Entity(AnyEntity))
+    requires IsSafe(r,s,e1,t1)
+    requires IsSafe(r,s,e2,Type.Set(t2))
+    requires forall u1, u2: EntityUID |
+      InstanceOfType(Value.EntityUID(u1), t1) && InstanceOfType(Value.EntityUID(u2), t2) ::
+      !EntityInEntity(s,u1,u2)
+    ensures IsFalse(r,s,BinaryApp(BinaryOp.In,e1,e2))
+  {
+    reveal IsSafe();
+    var evaluator := Evaluator(r,s);
+    var r1 := evaluator.interpret(e1);
+    var r2 := evaluator.interpret(e2);
+    if r1.Ok? && r2.Ok? {
+      var u1 := Value.asEntity(r1.value).value;
+      var s2 := Value.asSet(r2.value).value;
+      assert forall us2 <- s2 :: InstanceOfType(us2,t2);
+      var us2 :- assert evaluator.checkEntitySet(s2);
+      assert forall u2 <- us2 :: !EntityInEntity(s,u1,u2);
     }
   }
 }
